save

NuLLReps.thy
@@ -339,17 +339,6 @@ end
 
 subsection \<open>Fusion \<nu>-abstraction\<close>
 
-definition Fusion :: "('a1::lrep,'b1) \<nu> \<Rightarrow> ('a2::lrep,'b2) \<nu> \<Rightarrow> ('a1 \<times> 'a2, 'b1 \<times> 'b2) \<nu>" (infixr "\<nuFusion>" 70) 
-  where "Fusion N M p x = (case p of (p1,p2) \<Rightarrow> case x of (x1,x2) \<Rightarrow> (p1 \<nuLinkL> N \<nuLinkR> x1) \<and> (p2 \<nuLinkL> M \<nuLinkR> x2))"
-
-lemma [simp]: "(p1,p2) \<nuLinkL> N \<nuFusion> M \<nuLinkR> (x1,x2) \<longleftrightarrow> (p1 \<nuLinkL> N \<nuLinkR> x1) \<and> (p2 \<nuLinkL> M \<nuLinkR> x2)"
-  by (simp add: Fusion_def Refining_ex)
-lemma [elim,\<nu>elim]: "(x1,x2) \<ratio> N1 \<nuFusion> N2 \<Longrightarrow> (x1 \<ratio> N1 \<Longrightarrow> x2 \<ratio> N2 \<Longrightarrow> C) \<Longrightarrow> C" unfolding Inhabited_def by auto
-
-lemma [\<nu>intro]: "\<nu>Zero N z1 \<Longrightarrow> \<nu>Zero M z2 \<Longrightarrow> \<nu>Zero (N \<nuFusion> M) (z1,z2)" unfolding \<nu>Zero_def by simp
-
-lemma [\<nu>intro]: "\<^bold>c\<^bold>a\<^bold>s\<^bold>t x \<tycolon> N \<longmapsto> x' \<tycolon> N' \<^bold>w\<^bold>i\<^bold>t\<^bold>h P \<Longrightarrow> \<^bold>c\<^bold>a\<^bold>s\<^bold>t y \<tycolon> M \<longmapsto> y' \<tycolon> M' \<^bold>w\<^bold>i\<^bold>t\<^bold>h Q \<Longrightarrow>
-  \<^bold>c\<^bold>a\<^bold>s\<^bold>t (x,y) \<tycolon> N \<nuFusion> M \<longmapsto> (x',y') \<tycolon> N' \<nuFusion> M' \<^bold>w\<^bold>i\<^bold>t\<^bold>h P \<and> Q" unfolding Cast_def by auto
 
 definition AutoFusion (infixr "\<nuFusion>''" 70)  where "AutoFusion = Fusion"
 lemma [\<nu>intro]: "\<^bold>c\<^bold>a\<^bold>s\<^bold>t x \<tycolon> N \<nuFusion> M \<longmapsto> x' \<tycolon> N' \<nuFusion> M' \<^bold>w\<^bold>i\<^bold>t\<^bold>h P \<Longrightarrow> \<^bold>c\<^bold>a\<^bold>s\<^bold>t x \<tycolon> N \<nuFusion> M \<longmapsto> x' \<tycolon> N' \<nuFusion>' M' \<^bold>w\<^bold>i\<^bold>t\<^bold>h P"
