NuPrime.thy
@@ -159,6 +159,50 @@ lemma resource_key_exists: "Ex P \<longleftrightarrow> (\<exists>addr. P (MemAdd
 type_synonym heap = "resource_key \<rightharpoonup> deep_model"
 
 
+
+
+
+
+
+
+datatype com =
+  Basic " heap \<times> deep_model \<Rightarrow> heap \<times> deep_model"
+  | Seq com com
+  | Branch "com" "com"
+  | Until "com"
+
+inductive Sem :: "com \<Rightarrow> heap \<times> deep_model \<Rightarrow> heap \<times> deep_model \<Rightarrow> bool" where
+  "Sem (Basic f) s (f s)"
+| Sem_Seq:  "Sem f1 s s' \<Longrightarrow> Sem f2 s' s'' \<Longrightarrow> Sem (Seq f1 f2) s s'' "
+| "Sem f s (h, DM_fusion (DM_int 1 0) s') \<Longrightarrow> Sem (Until f) s (h, s')"
+| "Sem f s (h, DM_fusion (DM_int 1 1) s') \<Longrightarrow> Sem (Until f) (h,s') s'' \<Longrightarrow> Sem (Until f) s s''"
+
+inductive_cases AA[elim!]:
+  "Sem (Basic f) s s'" "Sem (Seq c1 c2) s s'"
+thm AA
+
+definition Proc :: " com \<Rightarrow> (heap \<times> deep_model) set \<Rightarrow> (heap \<times> deep_model) set \<Rightarrow> bool"
+  where "Proc f A B \<longleftrightarrow> (\<forall>x y. x \<in> A \<and> Sem f x y \<longrightarrow> y \<in> B)"
+
+lemma "Proc f A B \<Longrightarrow> Proc g B C \<Longrightarrow> Proc (Seq f g) A C"
+  unfolding Proc_def apply (auto intro: Sem_Seq)
+  by blast
+
+definition Ctx :: " heap set \<Rightarrow> deep_model set \<Rightarrow> (heap \<times> deep_model) set "
+  where "Ctx = (\<times>)"
+definition Fusion :: "(deep_model) set \<Rightarrow> (deep_model) set \<Rightarrow> (deep_model) set"
+  where "Fusion A B = { (DM_fusion a b) | a b. a \<in> A \<and> b \<in> B }"
+definition Boolean :: " bool \<Rightarrow> deep_model set"
+  where "Boolean b = { DM_int 1 (if b then 1 else 0) }"
+
+
+
+
+
+
+
+
+
 definition AvailableSegments :: "heap \<Rightarrow> msegment set"
   where "AvailableSegments heap = {seg. \<forall>ofs. heap (MemAddress (seg |+ ofs)) = None}"
 
@@ -208,7 +252,7 @@ subsubsection \<open>Definitions\<close>
 
 (* ceq : INF *)
 
-datatype ('a,'b) typing = typing 'b "('a,'b) \<nu>" ("_ \<tycolon> _" [16,16] 15) \<comment>\<open>shortcut keys "<ty>"\<close>
+datatype ('a,'b) typing = typing (typing_img: 'b ) (typing_nu: "('a,'b) \<nu>") ("_ \<tycolon> _" [16,16] 15) \<comment>\<open>shortcut keys "<ty>"\<close>
 primrec nu_of :: "('a,'b) typing \<Rightarrow> ('a,'b) \<nu>" where "nu_of (x \<tycolon> N) = N"
 primrec image_of :: "('a,'b) typing \<Rightarrow> 'b" where "image_of (x \<tycolon> N) = x"
 
@@ -216,7 +260,7 @@ definition RepSet :: "('a,'b) typing \<Rightarrow> 'a set" ("\<tort_lbrace> _ \<
 abbreviation Refining :: "'a \<Rightarrow> ('a,'b) \<nu> \<Rightarrow>  'b \<Rightarrow> bool" ("(_/ \<nuLinkL> _  \<nuLinkR>/ _)" [27,15,27] 26) \<comment>\<open>shortcut keys "--<" and ">--"\<close>
   where  "(p \<nuLinkL> N \<nuLinkR> x) \<equiv> p \<in> \<tort_lbrace>x \<tycolon> N\<tort_rbrace>"
 definition Inhabited :: " 'a set \<Rightarrow> bool" where "Inhabited s \<equiv> (\<exists>x. x \<in> s)"
-abbreviation InhabitTyp :: " 'b \<Rightarrow> ('a,'b) \<nu> \<Rightarrow> bool" ("_ \<ratio> _" [16,16] 15)  \<comment>\<open>shortcut keys ":TY:"\<close>
+abbreviation InhabitNu :: " 'b \<Rightarrow> ('a,'b) \<nu> \<Rightarrow> bool" ("_ \<ratio> _" [16,16] 15)  \<comment>\<open>shortcut keys ":TY:"\<close>
   where  " x \<ratio> N \<equiv> Inhabited \<tort_lbrace>x \<tycolon> N\<tort_rbrace>"
 text \<open>The @{term "x \<tycolon> N"} is a predication specifying concrete values,
   e.g. @{prop " a_concrete_int32 \<in> \<tort_lbrace>(42::nat) \<tycolon> N 32\<tort_rbrace>"} and also "state \<in> State (\<tort_lbrace>42 \<tycolon> N\<tort_rbrace> \<times> \<tort_lbrace>24 \<tycolon> N\<tort_rbrace> \<times> \<cdots> )".
@@ -331,66 +375,6 @@ subsection \<open>Stack structure\<close>
 class stack = lrep
 
 instantiation prod :: (lrep,stack) stack begin instance by standard end
-
-subsubsection \<open>Separation Conjecture\<close>
-
-definition disjoint :: " 'a set \<Rightarrow> 'a set \<Rightarrow> bool " (infixl "\<perpendicular>" 60) where "disjoint A B \<longleftrightarrow> (A \<inter> B = {})"
-lemma disjoint_rewL: "A \<perpendicular> B \<longleftrightarrow> (\<forall>x. x \<in> A \<longrightarrow> x \<notin> B)" unfolding disjoint_def by auto
-lemma disjoint_rewR: "A \<perpendicular> B \<longleftrightarrow> (\<forall>x. x \<in> B \<longrightarrow> x \<notin> A)" unfolding disjoint_def by auto
-
-lemma [iff]: "{} \<perpendicular> S" and [iff]: "S \<perpendicular> {}" unfolding disjoint_def by auto
-
-definition Separation :: " heap set \<Rightarrow> heap set \<Rightarrow> heap set" (infixl "\<heavy_asterisk>" 14)
-  where "Separation H1 H2 = {h. (\<exists>h1 h2. h = h1 ++ h2 \<and> dom h1 \<perpendicular> dom h2 \<and> h1 \<in> H1 \<and> h2 \<in> H2) }"
-definition NonSeparation :: " heap set \<Rightarrow> heap set \<Rightarrow> heap set" (infixl "\<dbl_and>" 13)
-  where "NonSeparation H1 H2 = {h. h \<in> H1 \<and> (\<exists>h'. h' \<subseteq>\<^sub>m h \<and> h' \<in> H2)}"
-
-translations
-  "H \<heavy_asterisk> x \<tycolon> T" == "H \<heavy_asterisk> \<tort_lbrace> x \<tycolon> T \<tort_rbrace>"
-  "x \<tycolon> T \<heavy_asterisk> H" == "\<tort_lbrace> x \<tycolon> T \<tort_rbrace> \<heavy_asterisk> H"
-  "H \<dbl_and> x \<tycolon> T" == "H \<dbl_and> \<tort_lbrace> x \<tycolon> T \<tort_rbrace>"
-  "x \<tycolon> T \<dbl_and> H" == "\<tort_lbrace> x \<tycolon> T \<tort_rbrace> \<dbl_and> H"
-
-lemma [iff]: "h \<in> (H1 \<heavy_asterisk> H2) \<longleftrightarrow> (\<exists>h1 h2. h = h1 ++ h2 \<and> dom h1 \<perpendicular> dom h2 \<and> h1 \<in> H1 \<and> h2 \<in> H2)" unfolding Separation_def by simp
-lemma [iff]: "h \<in> (H1 \<dbl_and> H2) \<longleftrightarrow> (h \<in> H1 \<and> (\<exists>h'. h' \<subseteq>\<^sub>m h \<and> h' \<in> H2))" unfolding NonSeparation_def by simp
-
-lemma [simp]: "A \<inter> S \<perpendicular> A \<inter> -S"
-  unfolding disjoint_def by auto
-lemma heap_split_id: "P h1' h2' \<Longrightarrow> \<exists>h1 h2. h1' ++ h2' = h1 ++ h2 \<and> P h1 h2" by auto
-lemma heap_split_by_set: "P (h |` S) (h |` (- S)) \<Longrightarrow> \<exists>h1 h2. h = h1 ++ h2 \<and> dom h1 \<perpendicular> dom h2 \<and> P h1 h2"
-  by (rule exI[of _ "h |` S"], rule exI[of _ "h |` (- S)"])
-    (auto simp add: map_add_def option.case_eq_if restrict_map_def disjoint_def disjoint_iff domIff)
-lemma heap_split_by_addr_set: "P (h |` (MemAddress ` S)) (h |` (- (MemAddress ` S))) \<Longrightarrow> \<exists>h1 h2. h = h1 ++ h2 \<and> dom h1 \<perpendicular> dom h2 \<and> P h1 h2"
-  using heap_split_by_set .
-
-lemma Separation_comm: "(P \<heavy_asterisk> Q) = (Q \<heavy_asterisk> P)"
-  by(auto simp add:Separation_def disjoint_def dest: map_add_comm)
-lemma Separation_assoc: "(A \<heavy_asterisk> (B \<heavy_asterisk> C)) = (A \<heavy_asterisk> B \<heavy_asterisk> C)"
-  by (auto simp add:Separation_def disjoint_def) 
-    (metis (no_types, lifting) Un_empty dom_map_add inf_sup_distrib1 inf_sup_distrib2 map_add_assoc)+
-
-lemma NonSeparation_distrib_L: "h \<in> (A \<heavy_asterisk> (B \<dbl_and> P)) \<Longrightarrow> h \<in> (A \<heavy_asterisk> B \<dbl_and> P)"
-  using map_le_map_add map_le_trans by blast
-lemma NonSeparation_distrib_R: "h \<in> ((A \<dbl_and> P) \<heavy_asterisk> B) \<Longrightarrow> h \<in> (A \<heavy_asterisk> B \<dbl_and> P)"
-  by (metis NonSeparation_distrib_L Separation_comm)
-  
-
-lemma [elim!,\<nu>elim]: "Inhabited (A \<heavy_asterisk> B) \<Longrightarrow> (Inhabited A \<Longrightarrow> Inhabited B \<Longrightarrow> C) \<Longrightarrow> C"
-  unfolding Inhabited_def by auto
-lemma [elim!,\<nu>elim]: "Inhabited (A \<dbl_and> B) \<Longrightarrow> (Inhabited A \<Longrightarrow> Inhabited B \<Longrightarrow> C) \<Longrightarrow> C"
-  unfolding Inhabited_def by auto
-
-subsubsection \<open>Delimiter operator\<close>
-
-definition Stack_Delimiter :: " ('a :: stack) set \<Rightarrow> ('b :: lrep) set \<Rightarrow> ('b \<times> 'a) set " ( "_/ \<heavy_comma> _" [14,15] 14)
-  where "Stack_Delimiter A B = (B \<times> A)"
-translations "R \<heavy_comma> x \<tycolon> N" == "R \<heavy_comma> \<tort_lbrace>x \<tycolon> N\<tort_rbrace>"
-  "x \<tycolon> N \<heavy_comma> R" == "\<tort_lbrace>x \<tycolon> N\<tort_rbrace> \<heavy_comma> R"
-
-lemma [simp]: " (a,b) \<in> (B \<heavy_comma> A) \<longleftrightarrow> a \<in> A \<and> b \<in> B" unfolding Stack_Delimiter_def by simp
-(* lemma [intro]: "[heap] a \<in>\<^sub>\<nu> A \<Longrightarrow> [heap] b \<in>\<^sub>\<nu> B \<Longrightarrow> [heap] (a,b) \<in>\<^sub>\<nu> (B \<heavy_comma> A)" by simp
-lemma [elim]: "[heap] ab \<in>\<^sub>\<nu> (B \<heavy_comma> A) \<Longrightarrow> (\<And>a b. ab = (a,b) \<Longrightarrow> [heap] a \<in>\<^sub>\<nu> A \<Longrightarrow> [heap] b \<in>\<^sub>\<nu> B \<Longrightarrow> C) \<Longrightarrow> C" by (cases ab) simp *)
-lemma [elim!,\<nu>elim]: "Inhabited (U\<heavy_comma>V) \<Longrightarrow> (Inhabited U \<Longrightarrow> Inhabited V \<Longrightarrow> C) \<Longrightarrow> C" unfolding Inhabited_def by auto
 
 subsubsection \<open>Context Type\<close>
 
@@ -634,228 +618,115 @@ lemma clean_user_facts:
 definition "SchemaTag x = x"
 (* translations "x" <= "CONST SchemaTag x" *)
 
-  subsubsection \<open>Existential Nu-type\<close>
+(* definition recursion :: "(('r \<longmapsto> 'r) \<Rightarrow> ('r \<longmapsto> 'r)) \<Rightarrow> 'r \<longmapsto> 'r"
+  where "recursion F s = (if (\<exists>s' R. wf R \<and> wfrec_rel R F s s'))"
 
-definition ExTyp :: "('a \<Rightarrow> 'b set) \<Rightarrow> 'b set" (binder "\<exists>* " 10)
-  where   "ExTyp T = {x. (\<exists>z. x \<in> T z)}"
-notation ExTyp (binder "\<exists>'' " 10)
-  \<comment> \<open>which represents there exists some \<nu>-images (or rarely abstractors) subject to the typing.
-    And then the image subjecting the typing could be fixed as a local variable by the \<nu>-obtain command. \<close>
-
-lemma [simp]: "x \<in> ExTyp T \<longleftrightarrow> (\<exists>z. x \<in> T z)" unfolding ExTyp_def  by auto
-lemma [simp]: "x \<in> \<S> (ExTyp T) \<longleftrightarrow> (\<exists>z. x \<in> \<S> (T z))" by (auto 4 3)
-lemma [simp]: "x \<in> \<S_S> (ExTyp T) \<longleftrightarrow> (\<exists>z. x \<in> \<S_S> (T z))" by (auto 4 3)
-lemma [simp]: "(ExTyp A \<heavy_comma> R) = (\<exists>* x. (A x \<heavy_comma> R))" by auto
-lemma [simp]: "(S\<heavy_comma> ExTyp T) = (\<exists>* z. (S \<heavy_comma> T z))" by auto
-lemma ExTyp_strip: "(\<^bold>c\<^bold>u\<^bold>r\<^bold>r\<^bold>e\<^bold>n\<^bold>t p \<^bold>r\<^bold>e\<^bold>s\<^bold>u\<^bold>l\<^bold>t\<^bold>s \<^bold>i\<^bold>n (ExTyp T)) \<equiv> (\<exists>x. \<^bold>c\<^bold>u\<^bold>r\<^bold>r\<^bold>e\<^bold>n\<^bold>t p \<^bold>r\<^bold>e\<^bold>s\<^bold>u\<^bold>l\<^bold>t\<^bold>s \<^bold>i\<^bold>n T x)"
-  unfolding CurrentConstruction_def by auto
+lemma t1: "wf R \<Longrightarrow> adm_wf R f \<Longrightarrow> wfrec_rel R f s s1 \<Longrightarrow> wfrec_rel R f s s2 \<Longrightarrow> s1 = s2"
+  using wfrec_unique by metis 
 
 
-(* definition AutoExTyp :: "('a \<Rightarrow> 'b set) \<Rightarrow> 'b set" (binder "\<exists>*''" 10)
-  where "AutoExTyp T = {x. (\<exists>z. x \<in> (T z))}"
-
-lemma [simp]: "x \<in> (AutoExTyp T) \<equiv> (\<exists>z. x \<in> T z)" unfolding AutoExTyp_def by auto
-lemma [simp]: "(R\<heavy_comma> AutoExTyp T) = (\<exists>*' x. (R\<heavy_comma> T x))" unfolding AutoExTyp_def by auto
-lemma [simp]: "(AutoExTyp T\<heavy_comma> R) = (\<exists>*' x. (T x\<heavy_comma> R))" unfolding AutoExTyp_def by auto
-lemma [simp]: "(AutoExTyp T \<flower> R) = (\<exists>*' x. (T x \<flower> R))" unfolding AutoExTyp_def BinderNameTag_def by auto
-
-lemma [simp]: "AutoExTyp T = (\<exists>*' a b. T (a,b))" unfolding AutoExTyp_def by auto
-
-lemma AutoExTyp_strip: "(\<^bold>c\<^bold>u\<^bold>r\<^bold>r\<^bold>e\<^bold>n\<^bold>t p \<^bold>r\<^bold>e\<^bold>s\<^bold>u\<^bold>l\<^bold>t\<^bold>s \<^bold>i\<^bold>n (AutoExTyp T)) \<equiv> (\<exists>x. \<^bold>c\<^bold>u\<^bold>r\<^bold>r\<^bold>e\<^bold>n\<^bold>t p \<^bold>r\<^bold>e\<^bold>s\<^bold>u\<^bold>l\<^bold>t\<^bold>s \<^bold>i\<^bold>n T x)"
-  unfolding AutoExTyp_def CurrentConstruction_def by (rule eq_reflection) auto *)
-
-  subsubsection \<open>Addition Nu-type : coheres true proposition\<close>
-
-definition AddtionTy :: " 'a set \<Rightarrow> bool \<Rightarrow> 'a set " (infixl "\<addition>" 50)
-  where " (T \<addition> P) = {x. x \<in> T \<and> P}"
-lemma [simp]: "T \<addition> True = T" unfolding AddtionTy_def by simp
-lemma [simp]: "x \<in> (T \<addition> P) \<longleftrightarrow> x \<in> T \<and> P" unfolding AddtionTy_def by simp
-(* lemma [intro]: "P \<Longrightarrow> [h] x \<in>\<^sub>\<nu> T \<Longrightarrow> [h] x \<in>\<^sub>\<nu> (T \<addition> P)" by simp
-lemma [elim]: "[h] x \<in>\<^sub>\<nu> (T \<addition> P) \<Longrightarrow> ([h] x \<in>\<^sub>\<nu> T \<Longrightarrow> P \<Longrightarrow> C) \<Longrightarrow> C" by simp*)
-lemma [simp]: "(R \<heavy_comma> T \<addition> P) = ((R \<heavy_comma> T) \<addition> P)" by auto
-lemma t1: "(\<^bold>c\<^bold>u\<^bold>r\<^bold>r\<^bold>e\<^bold>n\<^bold>t s \<^bold>r\<^bold>e\<^bold>s\<^bold>u\<^bold>l\<^bold>t\<^bold>s \<^bold>i\<^bold>n T \<addition> P) \<longleftrightarrow> (\<^bold>c\<^bold>u\<^bold>r\<^bold>r\<^bold>e\<^bold>n\<^bold>t s \<^bold>r\<^bold>e\<^bold>s\<^bold>u\<^bold>l\<^bold>t\<^bold>s \<^bold>i\<^bold>n T) \<and> P" unfolding CurrentConstruction_def by (cases s) auto
-lemma [simp]: "((((\<^bold>c\<^bold>u\<^bold>r\<^bold>r\<^bold>e\<^bold>n\<^bold>t s \<^bold>r\<^bold>e\<^bold>s\<^bold>u\<^bold>l\<^bold>t\<^bold>s \<^bold>i\<^bold>n S) \<and> B) \<and> C) \<^bold>w\<^bold>i\<^bold>t\<^bold>h \<^bold>f\<^bold>a\<^bold>c\<^bold>t\<^bold>s: PROP L) \<equiv> (((\<^bold>c\<^bold>u\<^bold>r\<^bold>r\<^bold>e\<^bold>n\<^bold>t s \<^bold>r\<^bold>e\<^bold>s\<^bold>u\<^bold>l\<^bold>t\<^bold>s \<^bold>i\<^bold>n S) \<and> (B \<and> C)) \<^bold>w\<^bold>i\<^bold>t\<^bold>h \<^bold>f\<^bold>a\<^bold>c\<^bold>t\<^bold>s: PROP L)" by simp
-
-lemma move_fact_to_star1[simp]:
-  "((\<^bold>c\<^bold>u\<^bold>r\<^bold>r\<^bold>e\<^bold>n\<^bold>t s \<^bold>r\<^bold>e\<^bold>s\<^bold>u\<^bold>l\<^bold>t\<^bold>s \<^bold>i\<^bold>n S \<addition> Q) \<^bold>w\<^bold>i\<^bold>t\<^bold>h \<^bold>f\<^bold>a\<^bold>c\<^bold>t\<^bold>s: PROP FactCollection (PROP NoFact) (PROP L) (PROP I))
-    \<Longrightarrow> (\<^bold>c\<^bold>u\<^bold>r\<^bold>r\<^bold>e\<^bold>n\<^bold>t s \<^bold>r\<^bold>e\<^bold>s\<^bold>u\<^bold>l\<^bold>t\<^bold>s \<^bold>i\<^bold>n S \<^bold>w\<^bold>i\<^bold>t\<^bold>h \<^bold>f\<^bold>a\<^bold>c\<^bold>t\<^bold>s: PROP FactCollection (Trueprop Q) (PROP L) (PROP I))"
-  unfolding t1 SpecTop_imp conj_imp FactCollection_imp
-  by (intro equal_intr_rule SpecTop_I FactCollection_I conjI NoFact) (* (unfold SpecTop_imp conj_imp FactCollection_imp) *)
-lemma move_fact_to_star2[simp]:
-  "((\<^bold>c\<^bold>u\<^bold>r\<^bold>r\<^bold>e\<^bold>n\<^bold>t s \<^bold>r\<^bold>e\<^bold>s\<^bold>u\<^bold>l\<^bold>t\<^bold>s \<^bold>i\<^bold>n S \<addition> Q) \<^bold>w\<^bold>i\<^bold>t\<^bold>h \<^bold>f\<^bold>a\<^bold>c\<^bold>t\<^bold>s: PROP FactCollection (Trueprop P) (PROP L) (PROP I))
-    \<Longrightarrow> (\<^bold>c\<^bold>u\<^bold>r\<^bold>r\<^bold>e\<^bold>n\<^bold>t s \<^bold>r\<^bold>e\<^bold>s\<^bold>u\<^bold>l\<^bold>t\<^bold>s \<^bold>i\<^bold>n S \<^bold>w\<^bold>i\<^bold>t\<^bold>h \<^bold>f\<^bold>a\<^bold>c\<^bold>t\<^bold>s: PROP FactCollection  (Trueprop (Q \<and> P)) (PROP L) (PROP I))"
-  unfolding t1 SpecTop_imp conj_imp FactCollection_imp
-  by (intro equal_intr_rule SpecTop_I FactCollection_I conjI) (* (unfold SpecTop_imp conj_imp FactCollection_imp) *)
-
-  subsection \<open>Cast\<close>
-
-definition Cast :: " 'a set \<Rightarrow> 'a set \<Rightarrow> bool \<Rightarrow> bool \<Rightarrow> bool " ("(2\<^bold>c\<^bold>a\<^bold>s\<^bold>t _ \<longmapsto> _/ \<^bold>w\<^bold>i\<^bold>t\<^bold>h _ \<^bold>w\<^bold>h\<^bold>e\<^bold>n _)" [13,13,13,13] 12)
-  where "(\<^bold>c\<^bold>a\<^bold>s\<^bold>t A \<longmapsto> B \<^bold>w\<^bold>i\<^bold>t\<^bold>h P \<^bold>w\<^bold>h\<^bold>e\<^bold>n Q) \<longleftrightarrow> (\<forall>v. Q \<longrightarrow> v \<in> A \<longrightarrow> v \<in> B \<and> P)"
-consts SimpleCast1 :: " 'a set \<Rightarrow> 'a set \<Rightarrow> bool \<Rightarrow> bool " ("(2\<^bold>c\<^bold>a\<^bold>s\<^bold>t _/ \<longmapsto> _ \<^bold>w\<^bold>i\<^bold>t\<^bold>h _)" [13,13,13] 12)
-consts SimpleCast2 :: " 'a set \<Rightarrow> 'a set \<Rightarrow> bool \<Rightarrow> bool " ("(2\<^bold>c\<^bold>a\<^bold>s\<^bold>t _/ \<longmapsto> _ \<^bold>w\<^bold>h\<^bold>e\<^bold>n _)" [13,13,13] 12)
-consts SimpleCast3 :: " 'a set \<Rightarrow> 'a set \<Rightarrow> bool " ("(2\<^bold>c\<^bold>a\<^bold>s\<^bold>t _/ \<longmapsto> _)" [13,13] 12)
-translations
-  "(\<^bold>c\<^bold>a\<^bold>s\<^bold>t A \<longmapsto> B)" == "(\<^bold>c\<^bold>a\<^bold>s\<^bold>t A \<longmapsto> B \<^bold>w\<^bold>i\<^bold>t\<^bold>h CONST True \<^bold>w\<^bold>h\<^bold>e\<^bold>n CONST True)"
-  "(\<^bold>c\<^bold>a\<^bold>s\<^bold>t A \<longmapsto> B \<^bold>w\<^bold>i\<^bold>t\<^bold>h P)" == "(\<^bold>c\<^bold>a\<^bold>s\<^bold>t A \<longmapsto> B \<^bold>w\<^bold>i\<^bold>t\<^bold>h P \<^bold>w\<^bold>h\<^bold>e\<^bold>n CONST True)"
-  "(\<^bold>c\<^bold>a\<^bold>s\<^bold>t A \<longmapsto> B \<^bold>w\<^bold>h\<^bold>e\<^bold>n P)" == "(\<^bold>c\<^bold>a\<^bold>s\<^bold>t A \<longmapsto> B \<^bold>w\<^bold>i\<^bold>t\<^bold>h CONST True \<^bold>w\<^bold>h\<^bold>e\<^bold>n P)"
-
-definition CastDual :: " 'a set \<Rightarrow> 'a set \<Rightarrow> bool \<Rightarrow> 'b set \<Rightarrow> 'b set \<Rightarrow> bool \<Rightarrow> bool " ("(2\<^bold>c\<^bold>a\<^bold>s\<^bold>t _/ \<longmapsto> _/ \<^bold>w\<^bold>i\<^bold>t\<^bold>h _/ \<^bold>d\<^bold>u\<^bold>a\<^bold>l _/ \<longmapsto> _/ \<^bold>w\<^bold>h\<^bold>e\<^bold>n _)" [13,13,13,13,13] 12)
-  where "CastDual A B P A' B' P' \<longleftrightarrow> (\<^bold>c\<^bold>a\<^bold>s\<^bold>t A \<longmapsto> B \<^bold>w\<^bold>i\<^bold>t\<^bold>h P) \<and> (\<^bold>c\<^bold>a\<^bold>s\<^bold>t A' \<longmapsto> B' \<^bold>w\<^bold>h\<^bold>e\<^bold>n P')"
-consts SimpCastDual1 :: " 'a set \<Rightarrow> 'a set \<Rightarrow> 'b set \<Rightarrow> 'b set \<Rightarrow> bool \<Rightarrow> bool " ("(2\<^bold>c\<^bold>a\<^bold>s\<^bold>t _/ \<longmapsto> _/ \<^bold>d\<^bold>u\<^bold>a\<^bold>l _/ \<longmapsto> _/ \<^bold>w\<^bold>h\<^bold>e\<^bold>n _)" [13,13,13,13] 12)
-consts SimpCastDual2 :: " 'a set \<Rightarrow> 'a set \<Rightarrow> bool \<Rightarrow> 'b set \<Rightarrow> 'b set \<Rightarrow> bool " ("(2\<^bold>c\<^bold>a\<^bold>s\<^bold>t _/ \<longmapsto> _/ \<^bold>w\<^bold>i\<^bold>t\<^bold>h _/ \<^bold>d\<^bold>u\<^bold>a\<^bold>l _/ \<longmapsto> _)" [13,13,13,13] 12)
-consts SimpCastDual3 :: " 'a set \<Rightarrow> 'a set \<Rightarrow> 'b set \<Rightarrow> 'b set \<Rightarrow> bool " ("(2\<^bold>c\<^bold>a\<^bold>s\<^bold>t _/ \<longmapsto> _/ \<^bold>d\<^bold>u\<^bold>a\<^bold>l _/ \<longmapsto> _)" [13,13,13] 12)
-translations
-  "\<^bold>c\<^bold>a\<^bold>s\<^bold>t A \<longmapsto> A' \<^bold>d\<^bold>u\<^bold>a\<^bold>l B \<longmapsto> B'" == "\<^bold>c\<^bold>a\<^bold>s\<^bold>t A \<longmapsto> A' \<^bold>w\<^bold>i\<^bold>t\<^bold>h CONST True \<^bold>d\<^bold>u\<^bold>a\<^bold>l B \<longmapsto> B' \<^bold>w\<^bold>h\<^bold>e\<^bold>n CONST True"
-  "\<^bold>c\<^bold>a\<^bold>s\<^bold>t A \<longmapsto> A' \<^bold>d\<^bold>u\<^bold>a\<^bold>l B \<longmapsto> B' \<^bold>w\<^bold>h\<^bold>e\<^bold>n Q" == "\<^bold>c\<^bold>a\<^bold>s\<^bold>t A \<longmapsto> A' \<^bold>w\<^bold>i\<^bold>t\<^bold>h CONST True \<^bold>d\<^bold>u\<^bold>a\<^bold>l B \<longmapsto> B' \<^bold>w\<^bold>h\<^bold>e\<^bold>n Q"
-  "\<^bold>c\<^bold>a\<^bold>s\<^bold>t A \<longmapsto> A' \<^bold>w\<^bold>i\<^bold>t\<^bold>h P \<^bold>d\<^bold>u\<^bold>a\<^bold>l B \<longmapsto> B'" == "\<^bold>c\<^bold>a\<^bold>s\<^bold>t A \<longmapsto> A' \<^bold>w\<^bold>i\<^bold>t\<^bold>h P \<^bold>d\<^bold>u\<^bold>a\<^bold>l B \<longmapsto> B' \<^bold>w\<^bold>h\<^bold>e\<^bold>n CONST True"
-
-translations
-  "\<^bold>c\<^bold>a\<^bold>s\<^bold>t x \<tycolon> X \<longmapsto> B \<^bold>w\<^bold>i\<^bold>t\<^bold>h P \<^bold>w\<^bold>h\<^bold>e\<^bold>n Q" == "\<^bold>c\<^bold>a\<^bold>s\<^bold>t \<tort_lbrace> x \<tycolon> X \<tort_rbrace> \<longmapsto> B \<^bold>w\<^bold>i\<^bold>t\<^bold>h P \<^bold>w\<^bold>h\<^bold>e\<^bold>n Q"
-  "\<^bold>c\<^bold>a\<^bold>s\<^bold>t A \<longmapsto> x \<tycolon> X \<^bold>w\<^bold>i\<^bold>t\<^bold>h P \<^bold>w\<^bold>h\<^bold>e\<^bold>n Q" == "\<^bold>c\<^bold>a\<^bold>s\<^bold>t A \<longmapsto> \<tort_lbrace> x \<tycolon> X \<tort_rbrace> \<^bold>w\<^bold>i\<^bold>t\<^bold>h P \<^bold>w\<^bold>h\<^bold>e\<^bold>n Q"
-  "\<^bold>c\<^bold>a\<^bold>s\<^bold>t A \<longmapsto> x \<tycolon> X \<^bold>w\<^bold>i\<^bold>t\<^bold>h P' \<^bold>d\<^bold>u\<^bold>a\<^bold>l A' \<longmapsto> B' \<^bold>w\<^bold>h\<^bold>e\<^bold>n P" == "\<^bold>c\<^bold>a\<^bold>s\<^bold>t A \<longmapsto> \<tort_lbrace>x \<tycolon> X\<tort_rbrace> \<^bold>w\<^bold>i\<^bold>t\<^bold>h P' \<^bold>d\<^bold>u\<^bold>a\<^bold>l A' \<longmapsto> B' \<^bold>w\<^bold>h\<^bold>e\<^bold>n P"
-  "\<^bold>c\<^bold>a\<^bold>s\<^bold>t a \<tycolon> A \<longmapsto> B \<^bold>w\<^bold>i\<^bold>t\<^bold>h P' \<^bold>d\<^bold>u\<^bold>a\<^bold>l A' \<longmapsto> B' \<^bold>w\<^bold>h\<^bold>e\<^bold>n P" == "\<^bold>c\<^bold>a\<^bold>s\<^bold>t \<tort_lbrace>a \<tycolon> A\<tort_rbrace> \<longmapsto> B \<^bold>w\<^bold>i\<^bold>t\<^bold>h P' \<^bold>d\<^bold>u\<^bold>a\<^bold>l A' \<longmapsto> B' \<^bold>w\<^bold>h\<^bold>e\<^bold>n P"
-  "\<^bold>c\<^bold>a\<^bold>s\<^bold>t A \<longmapsto> B \<^bold>w\<^bold>i\<^bold>t\<^bold>h P' \<^bold>d\<^bold>u\<^bold>a\<^bold>l a' \<tycolon> A' \<longmapsto> B' \<^bold>w\<^bold>h\<^bold>e\<^bold>n P" == "\<^bold>c\<^bold>a\<^bold>s\<^bold>t A \<longmapsto> B \<^bold>w\<^bold>i\<^bold>t\<^bold>h P' \<^bold>d\<^bold>u\<^bold>a\<^bold>l \<tort_lbrace>a' \<tycolon> A'\<tort_rbrace> \<longmapsto> B' \<^bold>w\<^bold>h\<^bold>e\<^bold>n P"
-  "\<^bold>c\<^bold>a\<^bold>s\<^bold>t A \<longmapsto> B \<^bold>w\<^bold>i\<^bold>t\<^bold>h P' \<^bold>d\<^bold>u\<^bold>a\<^bold>l A' \<longmapsto> b' \<tycolon> B' \<^bold>w\<^bold>h\<^bold>e\<^bold>n P" == "\<^bold>c\<^bold>a\<^bold>s\<^bold>t A \<longmapsto> B \<^bold>w\<^bold>i\<^bold>t\<^bold>h P' \<^bold>d\<^bold>u\<^bold>a\<^bold>l A' \<longmapsto> \<tort_lbrace>b' \<tycolon> B'\<tort_rbrace> \<^bold>w\<^bold>h\<^bold>e\<^bold>n P"
+lemma tt2:
+  assumes "wf R1" "wf R2" "adm_wf R1 F" "adm_wf R2 F"
+    "wfrec_rel R1 F s s1" "wfrec_rel R2 F s s2"
+  shows "s1 = s2"
+  using \<open>wf R1\<close> \<open>wf R2\<close>
+proof induct
+  define f1 where "f1 y = (THE z. wfrec_rel R1 F y z)" for y
+  case (less x)
+  then have "\<And>y z. (y, x) \<in> R1 \<Longrightarrow> wfrec_rel R1 F y z \<longleftrightarrow> z = f1 y"
+    unfolding f1_def by (rule theI_unique)
+  with \<open>adm_wf R F\<close> show ?case
+    by (subst wfrec_rel.simps) (auto simp: adm_wf_def)
+qed
 
 
-(* abbreviation SimpleCast :: " 'a set \<Rightarrow> 'a set \<Rightarrow> bool " ("(2\<^bold>c\<^bold>a\<^bold>s\<^bold>t _ \<longmapsto> _)" [2,14] 13)
-  where "(\<^bold>c\<^bold>a\<^bold>s\<^bold>t A \<longmapsto> B) \<equiv> (\<^bold>c\<^bold>a\<^bold>s\<^bold>t A \<longmapsto> B \<^bold>w\<^bold>i\<^bold>t\<^bold>h True)" *)
-(* lemma CastE[elim]: "\<^bold>c\<^bold>a\<^bold>s\<^bold>t A \<longmapsto> B \<^bold>w\<^bold>i\<^bold>t\<^bold>h P \<Longrightarrow> (\<not> Inhabited A \<Longrightarrow> C) \<Longrightarrow> (Inhabited A \<Longrightarrow> Inhabited B \<Longrightarrow> A \<subseteq> B \<Longrightarrow> P \<Longrightarrow> C) \<Longrightarrow> C"
-   unfolding Cast_def Inhabited_def by (auto intro: Inhabited_subset)
-lemma CastI[intro]: "Inhabited A \<Longrightarrow> A \<subseteq> B \<Longrightarrow> P \<Longrightarrow> \<^bold>c\<^bold>a\<^bold>s\<^bold>t A \<longmapsto> B \<^bold>w\<^bold>i\<^bold>t\<^bold>h P"
-  and [intro]: "\<not> Inhabited A \<Longrightarrow> \<^bold>c\<^bold>a\<^bold>s\<^bold>t A \<longmapsto> B \<^bold>w\<^bold>i\<^bold>t\<^bold>h P" unfolding Cast_def Inhabited_def by auto *)
-lemma cast_id[\<nu>intro0]: "\<^bold>c\<^bold>a\<^bold>s\<^bold>t A \<longmapsto> A" unfolding Cast_def by fast
-lemma cast_dual_id[\<nu>intro0]: "\<^bold>c\<^bold>a\<^bold>s\<^bold>t A \<longmapsto> A \<^bold>d\<^bold>u\<^bold>a\<^bold>l B \<longmapsto> B" unfolding CastDual_def  by (simp add: cast_id)
+term wfrec
+inductive SemRec :: "(('r \<longmapsto> 'r) \<Rightarrow> ('r \<longmapsto> 'r)) \<Rightarrow> heap \<times> 'r \<Rightarrow> 'r state \<Rightarrow> bool" where
+  "wf R \<Longrightarrow> adm_wf R f \<Longrightarrow> wfrec_rel R f s s' \<Longrightarrow> SemRec f s s' "
+lemma SemRec_deterministic:
+  assumes "SemRec c s s1"
+      and "SemRec c s s2"
+    shows "s1 = s2"
+proof -
+  have "SemRec c s s1 \<Longrightarrow> (\<forall>s2. SemRec c s s2 \<longrightarrow> s1 = s2)"
+    apply (induct rule: SemRec.induct)
+    apply (subst SemRec.simps)
+    using wfrec_unique
+    thm wfrec_unique
+    apply ( simp)+
+  thus ?thesis
+    using assms by simp
+qed
 
-lemma "=_\<nu>cast": "\<^bold>p\<^bold>a\<^bold>r\<^bold>a\<^bold>m x' \<Longrightarrow> \<^bold>p\<^bold>r\<^bold>e\<^bold>m\<^bold>i\<^bold>s\<^bold>e x = x' \<Longrightarrow> \<^bold>c\<^bold>a\<^bold>s\<^bold>t x \<tycolon> N \<longmapsto> x' \<tycolon> N" unfolding Cast_def by auto
-lemma [\<nu>intro']: "\<^bold>p\<^bold>r\<^bold>e\<^bold>m\<^bold>i\<^bold>s\<^bold>e N = N' \<Longrightarrow> \<^bold>p\<^bold>r\<^bold>e\<^bold>m\<^bold>i\<^bold>s\<^bold>e x = x' \<Longrightarrow> \<^bold>c\<^bold>a\<^bold>s\<^bold>t \<tort_lbrace>x \<tycolon> N\<tort_rbrace> \<longmapsto> \<tort_lbrace>x' \<tycolon> N'\<tort_rbrace>" unfolding Cast_def Premise_def by simp
-lemma [\<nu>intro0]: "\<^bold>p\<^bold>r\<^bold>e\<^bold>m\<^bold>i\<^bold>s\<^bold>e x = x" unfolding Premise_def by simp
-lemma [\<nu>intro]: " \<^bold>c\<^bold>a\<^bold>s\<^bold>t A \<longmapsto> A' \<^bold>w\<^bold>i\<^bold>t\<^bold>h P1 \<Longrightarrow> \<^bold>c\<^bold>a\<^bold>s\<^bold>t B \<longmapsto> B' \<^bold>w\<^bold>i\<^bold>t\<^bold>h P2 \<Longrightarrow> \<^bold>c\<^bold>a\<^bold>s\<^bold>t (A\<heavy_comma>B) \<longmapsto> (A'\<heavy_comma>B') \<^bold>w\<^bold>i\<^bold>t\<^bold>h P1 \<and> P2"
-  unfolding Cast_def by auto
 
-lemma cast_trans: "\<^bold>c\<^bold>a\<^bold>s\<^bold>t A \<longmapsto> B \<^bold>w\<^bold>i\<^bold>t\<^bold>h P \<Longrightarrow> \<^bold>c\<^bold>a\<^bold>s\<^bold>t B \<longmapsto> C \<^bold>w\<^bold>i\<^bold>t\<^bold>h Q \<Longrightarrow> \<^bold>c\<^bold>a\<^bold>s\<^bold>t A \<longmapsto> C \<^bold>w\<^bold>i\<^bold>t\<^bold>h P \<and> Q"
-  unfolding Cast_def by auto
-(* lemma dual_cast_fallback[\<nu>intro']: "\<^bold>c\<^bold>a\<^bold>s\<^bold>t A \<longmapsto> B \<^bold>w\<^bold>i\<^bold>t\<^bold>h P \<Longrightarrow> (\<^bold>c\<^bold>a\<^bold>s\<^bold>t A \<longmapsto> B) \<and> (\<^bold>c\<^bold>a\<^bold>s\<^bold>t C \<longmapsto> C)" unfolding Cast_def by fast *)
+thm SemRec.cases
 
-theorem apply_cast: "(\<^bold>c\<^bold>u\<^bold>r\<^bold>r\<^bold>e\<^bold>n\<^bold>t blk \<^bold>r\<^bold>e\<^bold>s\<^bold>u\<^bold>l\<^bold>t\<^bold>s \<^bold>i\<^bold>n (R \<heavy_comma> X\<heavy_comma> \<^bold>h\<^bold>e\<^bold>a\<^bold>p H)) \<Longrightarrow> (\<^bold>c\<^bold>a\<^bold>s\<^bold>t X \<longmapsto> Y \<^bold>w\<^bold>i\<^bold>t\<^bold>h P) \<Longrightarrow> (\<^bold>c\<^bold>u\<^bold>r\<^bold>r\<^bold>e\<^bold>n\<^bold>t blk \<^bold>r\<^bold>e\<^bold>s\<^bold>u\<^bold>l\<^bold>t\<^bold>s \<^bold>i\<^bold>n (R \<heavy_comma> Y\<heavy_comma> \<^bold>h\<^bold>e\<^bold>a\<^bold>p H) \<addition> P)"
-  unfolding Procedure_def CurrentConstruction_def PendingConstruction_def bind_def SpecTop_imp Cast_def by (auto 4 6)
-theorem cast: "\<^bold>c\<^bold>u\<^bold>r\<^bold>r\<^bold>e\<^bold>n\<^bold>t blk \<^bold>r\<^bold>e\<^bold>s\<^bold>u\<^bold>l\<^bold>t\<^bold>s \<^bold>i\<^bold>n T \<Longrightarrow> \<^bold>c\<^bold>a\<^bold>s\<^bold>t T \<longmapsto> T' \<^bold>w\<^bold>i\<^bold>t\<^bold>h P \<^bold>w\<^bold>h\<^bold>e\<^bold>n Q \<Longrightarrow> \<^bold>p\<^bold>r\<^bold>e\<^bold>m\<^bold>i\<^bold>s\<^bold>e Q \<Longrightarrow> \<^bold>c\<^bold>u\<^bold>r\<^bold>r\<^bold>e\<^bold>n\<^bold>t blk \<^bold>r\<^bold>e\<^bold>s\<^bold>u\<^bold>l\<^bold>t\<^bold>s \<^bold>i\<^bold>n T' "
-  for T' :: "(heap \<times> 'a::lrep) set" unfolding Cast_def CurrentConstruction_def by auto
+inductive SemUnt :: "('r \<longmapsto> bool \<times> 'r) \<Rightarrow> heap \<times> 'r \<Rightarrow> 'r state \<Rightarrow> bool" where
+  "f s = Success (h,False,r) \<Longrightarrow> SemUnt f s (Success (h,r))"
+| "f s = PartialCorrect \<Longrightarrow> SemUnt f s PartialCorrect"
+| "f s = Success (h,True,r) \<Longrightarrow> SemUnt f (h,r) s'' \<Longrightarrow> SemUnt f s s''"
 
-(* theorem proc_cast': "\<^bold>p\<^bold>r\<^bold>o\<^bold>c f \<blangle> A \<longmapsto> B \<brangle> \<Longrightarrow> \<^bold>c\<^bold>a\<^bold>s\<^bold>t A' \<longmapsto> A \<^bold>w\<^bold>i\<^bold>t\<^bold>h P \<Longrightarrow> \<^bold>c\<^bold>a\<^bold>s\<^bold>t B \<longmapsto> B' \<^bold>w\<^bold>i\<^bold>t\<^bold>h Q \<Longrightarrow> \<^bold>p\<^bold>r\<^bold>o\<^bold>c f \<blangle> A' \<longmapsto> B' \<brangle>"
-  unfolding Procedure_def Cast_def by (auto 0 4) *)
+lemma SemUnt_deterministic:
+  assumes "SemUnt c s s1"
+      and "SemUnt c s s2"
+    shows "s1 = s2"
+proof -
+  have "SemUnt c s s1 \<Longrightarrow> (\<forall>s2. SemUnt c s s2 \<longrightarrow> s1 = s2)"
+    by (induct rule: SemUnt.induct) (subst SemUnt.simps, simp)+
+  thus ?thesis
+    using assms by simp
+qed
 
-lemma [\<nu>intro']: "\<^bold>i\<^bold>n\<^bold>t\<^bold>r\<^bold>o \<^bold>c\<^bold>a\<^bold>s\<^bold>t A \<longmapsto> B \<^bold>w\<^bold>i\<^bold>t\<^bold>h P \<Longrightarrow> \<^bold>c\<^bold>a\<^bold>s\<^bold>t A \<longmapsto> B \<^bold>w\<^bold>i\<^bold>t\<^bold>h P" unfolding Intro_def .
-lemma [\<nu>intro']: "\<^bold>d\<^bold>e\<^bold>s\<^bold>t \<^bold>c\<^bold>a\<^bold>s\<^bold>t A \<longmapsto> B \<^bold>w\<^bold>i\<^bold>t\<^bold>h P \<Longrightarrow> \<^bold>c\<^bold>a\<^bold>s\<^bold>t A \<longmapsto> B \<^bold>w\<^bold>i\<^bold>t\<^bold>h P" unfolding Dest_def .
+definition Unt :: "('r \<longmapsto> bool \<times> 'r) \<Rightarrow> 'r \<longmapsto> 'r" where
+  "Unt f s = (if (\<exists>y. SemUnt f s y) then (THE y. SemUnt f s y) else PartialCorrect)"
 
-lemma "\<^bold>i\<^bold>n\<^bold>t\<^bold>r\<^bold>o \<^bold>c\<^bold>a\<^bold>s\<^bold>t A \<longmapsto> A" unfolding Intro_def using cast_id .
-lemma "\<^bold>d\<^bold>e\<^bold>s\<^bold>t \<^bold>c\<^bold>a\<^bold>s\<^bold>t A \<longmapsto> A" unfolding Dest_def using cast_id .
-  \<comment> \<open>All intro-cast or dest-cast involved in the reasoner constitute a directed acyclic graph WITH self-loop.
-    Note the self-loop has the lowest priority, so that the self-loop only be tried ONCE in the whole reasoning
-      (when all other rules cannot be applied), and only longest inference chains (who cannot be extended by
-      any other rules) will be tried by self-loop.
-    \<^term>\<open>Different\<close> can be used to assert the non-self-loop.\<close>
+lemma "\<exists>until. "
 
-subsection \<open>Conversion\<close>
 
-(* definition AutoTag :: "bool \<Rightarrow> bool" ("\<^bold>a\<^bold>u\<^bold>t\<^bold>o _" [100] 99) where [\<nu>def]: "\<^bold>a\<^bold>u\<^bold>t\<^bold>o P \<longleftrightarrow> P"
-lemma [\<nu>intro]: "[heap] \<^bold>c\<^bold>a\<^bold>s\<^bold>t U \<longmapsto> U' \<Longrightarrow> \<^bold>a\<^bold>u\<^bold>t\<^bold>o \<^bold>p\<^bold>r\<^bold>o\<^bold>c nop \<blangle> U \<longmapsto> U' \<brangle>"
-  unfolding AutoTag_def Cast_def Procedure_def nop_def by auto *)
-  
-definition Conversion :: "('a::lrep \<longmapsto> 'b::lrep) \<Rightarrow> (heap\<times>'a) set \<Rightarrow> (heap\<times>'b) set \<Rightarrow> ( ('c::lrep) \<longmapsto> ('d::lrep)) \<Rightarrow> (heap\<times>'c) set \<Rightarrow> (heap\<times>'d) set \<Rightarrow> bool"
-    ("\<^bold>c\<^bold>o\<^bold>n\<^bold>v\<^bold>e\<^bold>r\<^bold>s\<^bold>i\<^bold>o\<^bold>n _/ (2\<blangle> _/ \<longmapsto> _ \<brangle>)/ \<long_dobule_mapsto> _/ (2\<blangle> _/ \<longmapsto> _ \<brangle>)" [101,2,2,101,2,2] 100)
-    where [\<nu>def]: "\<^bold>c\<^bold>o\<^bold>n\<^bold>v\<^bold>e\<^bold>r\<^bold>s\<^bold>i\<^bold>o\<^bold>n f \<blangle> U \<longmapsto> V \<brangle> \<long_dobule_mapsto> g \<blangle> U' \<longmapsto> V' \<brangle> \<longleftrightarrow>( \<^bold>p\<^bold>r\<^bold>o\<^bold>c f \<blangle> U \<longmapsto> V \<brangle> \<longrightarrow> \<^bold>p\<^bold>r\<^bold>o\<^bold>c g \<blangle> U' \<longmapsto> V' \<brangle> )"
 
-lemma conversion: "\<^bold>c\<^bold>o\<^bold>n\<^bold>v\<^bold>e\<^bold>r\<^bold>s\<^bold>i\<^bold>o\<^bold>n f \<blangle> U \<longmapsto> V \<brangle> \<long_dobule_mapsto> f' \<blangle> U' \<longmapsto> V' \<brangle> \<Longrightarrow> \<^bold>p\<^bold>r\<^bold>o\<^bold>c f \<blangle> U \<longmapsto> V \<brangle> \<Longrightarrow> \<^bold>p\<^bold>r\<^bold>o\<^bold>c f' \<blangle> U' \<longmapsto> V' \<brangle>"
-  for f :: " ('a::lrep) \<longmapsto> ('b::lrep)" and f' :: " ('c::lrep) \<longmapsto> ('d::lrep)" unfolding Conversion_def by fast
+datatype com =
+  Basic " heap \<times> deep_model \<Rightarrow> heap \<times> deep_model"
+  | Seq com com
+  | Branch "com" "com"
+  | Until "com"
 
-lemma [\<nu>intro0]: "\<^bold>c\<^bold>o\<^bold>n\<^bold>v\<^bold>e\<^bold>r\<^bold>s\<^bold>i\<^bold>o\<^bold>n f \<blangle> U \<longmapsto> V \<brangle> \<long_dobule_mapsto> f \<blangle> U \<longmapsto> V \<brangle>" unfolding Conversion_def by fast
+inductive Sem :: "com \<Rightarrow> heap \<times> deep_model \<Rightarrow> heap \<times> deep_model \<Rightarrow> bool" where
+  "Sem (Basic f) s (f s)"
+| "Sem f1 s s' \<Longrightarrow> Sem f2 s' s'' \<Longrightarrow> Sem (Seq f1 f2) s s'' "
+| "Sem f s (h, DM_fusion (DM_int 1 0) s') \<Longrightarrow> Sem (Until f) s (h, s')"
+| "Sem f s (h, DM_fusion (DM_int 1 1) s') \<Longrightarrow> Sem (Until f) (h,s') s'' \<Longrightarrow> Sem (Until f) s s''"
 
-lemma conversion_cast[\<nu>intro]: "\<^bold>c\<^bold>a\<^bold>s\<^bold>t U' \<longmapsto> U \<^bold>w\<^bold>i\<^bold>t\<^bold>h P \<^bold>d\<^bold>u\<^bold>a\<^bold>l V \<longmapsto> V' \<^bold>w\<^bold>h\<^bold>e\<^bold>n Q \<Longrightarrow> \<^bold>p\<^bold>r\<^bold>e\<^bold>m\<^bold>i\<^bold>s\<^bold>e (P \<longrightarrow> Q) \<Longrightarrow> \<^bold>c\<^bold>o\<^bold>n\<^bold>v\<^bold>e\<^bold>r\<^bold>s\<^bold>i\<^bold>o\<^bold>n f \<blangle> U \<longmapsto> V \<brangle> \<long_dobule_mapsto> f \<blangle> U' \<longmapsto> V'\<brangle>"
-  unfolding Conversion_def Procedure_def Cast_def CastDual_def id_def
-  by (metis Cast_def CurrentConstruction_def LooseStateTy_introByStrict LooseStateTy_upgrade Premise_def cast)
-(* lemma [\<nu>intro]: "\<^bold>p\<^bold>r\<^bold>o\<^bold>c g \<blangle> U' \<longmapsto> U \<brangle> \<Longrightarrow> \<^bold>c\<^bold>o\<^bold>n\<^bold>v\<^bold>e\<^bold>r\<^bold>s\<^bold>i\<^bold>o\<^bold>n f \<blangle> U \<longmapsto> V \<brangle> \<long_dobule_mapsto> (g \<nuInstrComp> f) \<blangle> U' \<longmapsto> V\<brangle>"
-  unfolding Conversion_def using instr_comp by fast *)
 
-theorem apply_proc_conv: "(\<^bold>c\<^bold>u\<^bold>r\<^bold>r\<^bold>e\<^bold>n\<^bold>t blk \<^bold>r\<^bold>e\<^bold>s\<^bold>u\<^bold>l\<^bold>t\<^bold>s \<^bold>i\<^bold>n S) \<Longrightarrow> (\<^bold>c\<^bold>o\<^bold>n\<^bold>v\<^bold>e\<^bold>r\<^bold>s\<^bold>i\<^bold>o\<^bold>n f \<blangle> S' \<longmapsto> T' \<brangle> \<long_dobule_mapsto> g \<blangle> S \<longmapsto> T\<brangle>) \<Longrightarrow> \<^bold>p\<^bold>r\<^bold>o\<^bold>c f \<blangle> S' \<longmapsto> T' \<brangle> \<Longrightarrow> (\<^bold>p\<^bold>e\<^bold>n\<^bold>d\<^bold>i\<^bold>n\<^bold>g g \<^bold>o\<^bold>n blk \<^bold>r\<^bold>e\<^bold>s\<^bold>u\<^bold>l\<^bold>t\<^bold>s \<^bold>i\<^bold>n T)"
-  unfolding Procedure_def CurrentConstruction_def PendingConstruction_def bind_def SpecTop_imp Conversion_def by auto
+end
+codatatype 'a colist = conil | cocons 'a " 'a colist "
+primcorec "from" where "from n  = cocons n (from (Suc n))"
+thm colist.coinduct
+coinductive infinite where
+  Inf: "infinite l \<Longrightarrow> infinite (cocons x l)"
+thm infinite.coinduct
+lemma "infinite (from n)"
+  apply (coinduct rule: infinite.coinduct[of "\<lambda>x. \<exists>n. x = from n "])
+   apply auto
+  using from.code by blast 
 
-lemma conversion_trans: "\<^bold>c\<^bold>o\<^bold>n\<^bold>v\<^bold>e\<^bold>r\<^bold>s\<^bold>i\<^bold>o\<^bold>n g \<blangle> Xg \<longmapsto> Yg \<brangle> \<long_dobule_mapsto> h \<blangle> Xh \<longmapsto> Yh \<brangle>
-  \<Longrightarrow> \<^bold>c\<^bold>o\<^bold>n\<^bold>v\<^bold>e\<^bold>r\<^bold>s\<^bold>i\<^bold>o\<^bold>n f \<blangle> Xf \<longmapsto> Yf \<brangle> \<long_dobule_mapsto> g \<blangle> Xg \<longmapsto> Yg \<brangle>
-  \<Longrightarrow> \<^bold>c\<^bold>o\<^bold>n\<^bold>v\<^bold>e\<^bold>r\<^bold>s\<^bold>i\<^bold>o\<^bold>n f \<blangle> Xf \<longmapsto> Yf\<brangle> \<long_dobule_mapsto> h \<blangle> Xh \<longmapsto> Yh \<brangle>"
-  unfolding Conversion_def by blast
+  subgoal premises _ for x
+  apply clarify
+  thm from_def
+  thm infinite.coinduct
 
-subsection \<open>Heap\<close>
 
-consts ResourceState :: " heap \<Rightarrow> 'a \<Rightarrow> 'b set \<Rightarrow> bool" ("_ \<^bold>a\<^bold>t _ \<^bold>i\<^bold>s _ " [16,16,12] 11)
-consts allocated :: " heap \<Rightarrow> 'a \<Rightarrow> bool"
+datatype ENat =  N | S  ENat
 
-translations "h \<^bold>a\<^bold>t resource \<^bold>i\<^bold>s x \<tycolon> T" \<rightleftharpoons> "h \<^bold>a\<^bold>t resource \<^bold>i\<^bold>s \<tort_lbrace> x \<tycolon> T \<tort_rbrace>"
+primrec min where
+  "min N _ = N" | "min _ N = N" | "min (S n) (S m) = min n m"
+   "min n m = (case n of
+       N \<Rightarrow> N
+     | S n' \<Rightarrow> (case m of
+        N \<Rightarrow> N
+      | S m' \<Rightarrow> S (min n' m')))"
 
-definition "addr_allocated heap addr \<longleftrightarrow> MemAddress addr \<in> dom heap"
-adhoc_overloading allocated addr_allocated
-
-(* lemma addr_allocated_mono[dest]: "h \<subseteq>\<^sub>m h' \<Longrightarrow> addr_allocated h addr \<Longrightarrow> addr_allocated h' addr"
-  unfolding addr_allocated_def by auto
-lemma [iff]: "addr_allocated (h(k \<mapsto> v)) addr \<longleftrightarrow> k = MemAddress addr \<or> addr_allocated h addr"
-  and [iff]: "addr_allocated (h(k := None)) addr \<longleftrightarrow> k \<noteq> MemAddress addr \<and> addr_allocated h addr"
-  unfolding addr_allocated_def by auto *)
-lemma [iff]: "addr_allocated (h(k \<mapsto> v)) addr \<longleftrightarrow> k = MemAddress addr \<or> addr_allocated h addr"
-  and [iff]: "addr_allocated (h(k := None)) addr \<longleftrightarrow> k \<noteq> MemAddress addr \<and> addr_allocated h addr"
-  unfolding addr_allocated_def by auto
-
-definition MemAddrState :: "heap \<Rightarrow> nat memaddr \<Rightarrow> 'b::lrep set \<Rightarrow> bool"
-  where "MemAddrState h addr S \<longleftrightarrow> addr_allocated h addr \<and> shallowize (the (h (MemAddress addr))) \<in> S"
-adhoc_overloading ResourceState MemAddrState
-
-(*lemma MemAddrState_mono[dest]: "h \<subseteq>\<^sub>m h' \<Longrightarrow> MemAddrState h addr S \<Longrightarrow> MemAddrState h' addr S"
-  unfolding MemAddrState_def addr_allocated_def by auto (metis \<nu>set_mono domI map_le_def option.sel) *)
-
-lemma MemAddrState_I_neq[intro]: "k2 \<noteq> k \<Longrightarrow> MemAddrState h k2 S \<Longrightarrow> MemAddrState (h(MemAddress k := v)) k2 S"
-  and MemAddrState_I_eq[intro]: "v' \<in> S \<Longrightarrow> MemAddrState (h(MemAddress k \<mapsto> deepize v')) k S"
-  unfolding MemAddrState_def addr_allocated_def by auto
-
-lemma MemAddrState_E[elim]:
-  "MemAddrState h addr S \<Longrightarrow> (addr_allocated h addr \<Longrightarrow> Inhabited S \<Longrightarrow> C) \<Longrightarrow> C"
-  unfolding MemAddrState_def by auto
-lemma MemAddrState_I:
-  "addr_allocated h addr \<Longrightarrow> shallowize (the (h (MemAddress addr))) \<in> S \<Longrightarrow> MemAddrState h addr S"
-  unfolding MemAddrState_def by auto
-
-(* lemma MemAddrState_retained_N[intro]:
-  "k \<noteq> MemAddress addr \<Longrightarrow> MemAddrState h addr S \<Longrightarrow> \<nu>Independent S claim
-    \<Longrightarrow> Alive k \<in> claim \<Longrightarrow> MemAddrState (h(k:=None)) addr S"
-  unfolding MemAddrState_def \<nu>Independent_def by auto
-lemma MemAddrState_retained_S[intro]:
-  "k \<noteq> MemAddress addr \<Longrightarrow> MemAddrState h addr S \<Longrightarrow> \<nu>Independent S claim
-    \<Longrightarrow> Write k \<in> claim \<Longrightarrow> MemAddrState (h(k \<mapsto> v)) addr S"
-  unfolding MemAddrState_def \<nu>Independent_def by auto
-
+coinductive le where
+  leN: "le N m"
+| leS: "le n m \<Longrightarrow> le (S n) (S m)"
 *)
-
-
-lemma MemAddrState_restrict_I1[intro]: "h \<^bold>a\<^bold>t a \<^bold>i\<^bold>s T \<Longrightarrow> a \<in> S \<Longrightarrow> h |` (MemAddress ` S) \<^bold>a\<^bold>t a \<^bold>i\<^bold>s T "
-  and MemAddrState_restrict_I2[intro]: "h \<^bold>a\<^bold>t a \<^bold>i\<^bold>s T \<Longrightarrow> a \<notin> S \<Longrightarrow> h |` (- MemAddress ` S) \<^bold>a\<^bold>t a \<^bold>i\<^bold>s T "
-  unfolding MemAddrState_def addr_allocated_def
-  by auto (metis ComplI imageE option.sel resource_key.inject(1) restrict_map_def)
-
-lemma MemAddrState_add_I1[intro]: " h1 \<^bold>a\<^bold>t a \<^bold>i\<^bold>s T \<Longrightarrow> dom h1 \<perpendicular> dom h2 \<Longrightarrow> h1 ++ h2 \<^bold>a\<^bold>t a \<^bold>i\<^bold>s T "
-  and  MemAddrState_add_I2[intro]: " h2 \<^bold>a\<^bold>t a \<^bold>i\<^bold>s T \<Longrightarrow> dom h1 \<perpendicular> dom h2 \<Longrightarrow> h1 ++ h2 \<^bold>a\<^bold>t a \<^bold>i\<^bold>s T "
-  unfolding MemAddrState_def addr_allocated_def by (auto simp add: map_add_def disjoint_def split: option.split)
-  
-
- subsubsection \<open>Auto construct & destruct\<close>
-
-definition AutoConstruct :: " 'exp \<Rightarrow> ('a::lrep \<longmapsto> 'b::lrep) \<Rightarrow> (heap \<times> 'a) set \<Rightarrow> (heap \<times> 'b) set \<Rightarrow> bool "("\<^bold>c\<^bold>o\<^bold>n\<^bold>s\<^bold>t\<^bold>r\<^bold>u\<^bold>c\<^bold>t _/ \<^bold>b\<^bold>y \<^bold>p\<^bold>r\<^bold>o\<^bold>c _/ (2\<blangle>_/ \<longmapsto> _ \<brangle>)" [20,101,10,10] 100)
-  where [\<nu>def]:"AutoConstruct exp f S T \<longleftrightarrow> \<^bold>p\<^bold>r\<^bold>o\<^bold>c f \<blangle> S \<longmapsto> T \<brangle>"
-lemma AutoConstruct: "(\<^bold>c\<^bold>u\<^bold>r\<^bold>r\<^bold>e\<^bold>n\<^bold>t blk \<^bold>r\<^bold>e\<^bold>s\<^bold>u\<^bold>l\<^bold>t\<^bold>s \<^bold>i\<^bold>n S) \<Longrightarrow> AutoConstruct exp f S T \<Longrightarrow> (\<^bold>p\<^bold>e\<^bold>n\<^bold>d\<^bold>i\<^bold>n\<^bold>g f \<^bold>o\<^bold>n blk \<^bold>r\<^bold>e\<^bold>s\<^bold>u\<^bold>l\<^bold>t\<^bold>s \<^bold>i\<^bold>n T)" for exp :: "'exp"
-  unfolding AutoConstruct_def using apply_proc .
-
-(* lemma [simp]: "(Inhabited A \<and> Inhabited B) \<or> (Inhabited A' \<and> Inhabited B')
-  \<Longrightarrow> (A\<heavy_comma>B) = (A'\<heavy_comma>B') \<longleftrightarrow> A = A' \<and> B = B'" unfolding Stack_Delimiter_def Inhabited_def by (auto simp add: times_eq_iff) 
-lemma  [elim]: "(A\<heavy_comma>B) = (A'\<heavy_comma>B') \<Longrightarrow> (A = {} \<or> B = {} \<Longrightarrow> A' = {} \<or> B' = {} \<Longrightarrow> C) \<Longrightarrow> (A = A' \<Longrightarrow> B = B' \<Longrightarrow> C) \<Longrightarrow> C"
-  unfolding Stack_Delimiter_def by (auto simp add: times_eq_iff)
-*)
-
-
 end
