NuSys.thy
@@ -29,6 +29,231 @@ definition  FailedPremise :: "bool \<Rightarrow> bool" where "FailedPremise \<eq
 lemma FailedPremise_I: "\<^bold>p\<^bold>r\<^bold>e\<^bold>m\<^bold>i\<^bold>s\<^bold>e P \<Longrightarrow> FailedPremise P" unfolding FailedPremise_def .
 lemma FailedPremise_D: "FailedPremise P \<Longrightarrow> \<^bold>p\<^bold>r\<^bold>e\<^bold>m\<^bold>i\<^bold>s\<^bold>e P" unfolding FailedPremise_def .
 
+section \<open>Mechanisms - I\<close>
+
+  subsection \<open>Cast\<close>
+
+definition Cast :: " 'a set \<Rightarrow> 'a set \<Rightarrow> bool \<Rightarrow> bool \<Rightarrow> bool " ("(2\<^bold>c\<^bold>a\<^bold>s\<^bold>t _ \<longmapsto> _/ \<^bold>w\<^bold>i\<^bold>t\<^bold>h _ \<^bold>w\<^bold>h\<^bold>e\<^bold>n _)" [13,13,13,13] 12)
+  where "(\<^bold>c\<^bold>a\<^bold>s\<^bold>t A \<longmapsto> B \<^bold>w\<^bold>i\<^bold>t\<^bold>h P \<^bold>w\<^bold>h\<^bold>e\<^bold>n Q) \<longleftrightarrow> (\<forall>v. Q \<longrightarrow> v \<in> A \<longrightarrow> v \<in> B \<and> P)"
+consts SimpleCast1 :: " 'a set \<Rightarrow> 'a set \<Rightarrow> bool \<Rightarrow> bool " ("(2\<^bold>c\<^bold>a\<^bold>s\<^bold>t _/ \<longmapsto> _ \<^bold>w\<^bold>i\<^bold>t\<^bold>h _)" [13,13,13] 12)
+consts SimpleCast2 :: " 'a set \<Rightarrow> 'a set \<Rightarrow> bool \<Rightarrow> bool " ("(2\<^bold>c\<^bold>a\<^bold>s\<^bold>t _/ \<longmapsto> _ \<^bold>w\<^bold>h\<^bold>e\<^bold>n _)" [13,13,13] 12)
+consts SimpleCast3 :: " 'a set \<Rightarrow> 'a set \<Rightarrow> bool " ("(2\<^bold>c\<^bold>a\<^bold>s\<^bold>t _/ \<longmapsto> _)" [13,13] 12)
+translations
+  "(\<^bold>c\<^bold>a\<^bold>s\<^bold>t A \<longmapsto> B)" == "(\<^bold>c\<^bold>a\<^bold>s\<^bold>t A \<longmapsto> B \<^bold>w\<^bold>i\<^bold>t\<^bold>h CONST True \<^bold>w\<^bold>h\<^bold>e\<^bold>n CONST True)"
+  "(\<^bold>c\<^bold>a\<^bold>s\<^bold>t A \<longmapsto> B \<^bold>w\<^bold>i\<^bold>t\<^bold>h P)" == "(\<^bold>c\<^bold>a\<^bold>s\<^bold>t A \<longmapsto> B \<^bold>w\<^bold>i\<^bold>t\<^bold>h P \<^bold>w\<^bold>h\<^bold>e\<^bold>n CONST True)"
+  "(\<^bold>c\<^bold>a\<^bold>s\<^bold>t A \<longmapsto> B \<^bold>w\<^bold>h\<^bold>e\<^bold>n P)" == "(\<^bold>c\<^bold>a\<^bold>s\<^bold>t A \<longmapsto> B \<^bold>w\<^bold>i\<^bold>t\<^bold>h CONST True \<^bold>w\<^bold>h\<^bold>e\<^bold>n P)"
+
+definition CastDual :: " 'a set \<Rightarrow> 'a set \<Rightarrow> bool \<Rightarrow> 'b set \<Rightarrow> 'b set \<Rightarrow> bool \<Rightarrow> bool " ("(2\<^bold>c\<^bold>a\<^bold>s\<^bold>t _/ \<longmapsto> _/ \<^bold>w\<^bold>i\<^bold>t\<^bold>h _/ \<^bold>d\<^bold>u\<^bold>a\<^bold>l _/ \<longmapsto> _/ \<^bold>w\<^bold>h\<^bold>e\<^bold>n _)" [13,13,13,13,13] 12)
+  where "CastDual A B P A' B' P' \<longleftrightarrow> (\<^bold>c\<^bold>a\<^bold>s\<^bold>t A \<longmapsto> B \<^bold>w\<^bold>i\<^bold>t\<^bold>h P) \<and> (\<^bold>c\<^bold>a\<^bold>s\<^bold>t A' \<longmapsto> B' \<^bold>w\<^bold>h\<^bold>e\<^bold>n P')"
+consts SimpCastDual1 :: " 'a set \<Rightarrow> 'a set \<Rightarrow> 'b set \<Rightarrow> 'b set \<Rightarrow> bool \<Rightarrow> bool " ("(2\<^bold>c\<^bold>a\<^bold>s\<^bold>t _/ \<longmapsto> _/ \<^bold>d\<^bold>u\<^bold>a\<^bold>l _/ \<longmapsto> _/ \<^bold>w\<^bold>h\<^bold>e\<^bold>n _)" [13,13,13,13] 12)
+consts SimpCastDual2 :: " 'a set \<Rightarrow> 'a set \<Rightarrow> bool \<Rightarrow> 'b set \<Rightarrow> 'b set \<Rightarrow> bool " ("(2\<^bold>c\<^bold>a\<^bold>s\<^bold>t _/ \<longmapsto> _/ \<^bold>w\<^bold>i\<^bold>t\<^bold>h _/ \<^bold>d\<^bold>u\<^bold>a\<^bold>l _/ \<longmapsto> _)" [13,13,13,13] 12)
+consts SimpCastDual3 :: " 'a set \<Rightarrow> 'a set \<Rightarrow> 'b set \<Rightarrow> 'b set \<Rightarrow> bool " ("(2\<^bold>c\<^bold>a\<^bold>s\<^bold>t _/ \<longmapsto> _/ \<^bold>d\<^bold>u\<^bold>a\<^bold>l _/ \<longmapsto> _)" [13,13,13] 12)
+translations
+  "\<^bold>c\<^bold>a\<^bold>s\<^bold>t A \<longmapsto> A' \<^bold>d\<^bold>u\<^bold>a\<^bold>l B \<longmapsto> B'" == "\<^bold>c\<^bold>a\<^bold>s\<^bold>t A \<longmapsto> A' \<^bold>w\<^bold>i\<^bold>t\<^bold>h CONST True \<^bold>d\<^bold>u\<^bold>a\<^bold>l B \<longmapsto> B' \<^bold>w\<^bold>h\<^bold>e\<^bold>n CONST True"
+  "\<^bold>c\<^bold>a\<^bold>s\<^bold>t A \<longmapsto> A' \<^bold>d\<^bold>u\<^bold>a\<^bold>l B \<longmapsto> B' \<^bold>w\<^bold>h\<^bold>e\<^bold>n Q" == "\<^bold>c\<^bold>a\<^bold>s\<^bold>t A \<longmapsto> A' \<^bold>w\<^bold>i\<^bold>t\<^bold>h CONST True \<^bold>d\<^bold>u\<^bold>a\<^bold>l B \<longmapsto> B' \<^bold>w\<^bold>h\<^bold>e\<^bold>n Q"
+  "\<^bold>c\<^bold>a\<^bold>s\<^bold>t A \<longmapsto> A' \<^bold>w\<^bold>i\<^bold>t\<^bold>h P \<^bold>d\<^bold>u\<^bold>a\<^bold>l B \<longmapsto> B'" == "\<^bold>c\<^bold>a\<^bold>s\<^bold>t A \<longmapsto> A' \<^bold>w\<^bold>i\<^bold>t\<^bold>h P \<^bold>d\<^bold>u\<^bold>a\<^bold>l B \<longmapsto> B' \<^bold>w\<^bold>h\<^bold>e\<^bold>n CONST True"
+
+translations
+  "\<^bold>c\<^bold>a\<^bold>s\<^bold>t x \<tycolon> X \<longmapsto> B \<^bold>w\<^bold>i\<^bold>t\<^bold>h P \<^bold>w\<^bold>h\<^bold>e\<^bold>n Q" == "\<^bold>c\<^bold>a\<^bold>s\<^bold>t \<tort_lbrace> x \<tycolon> X \<tort_rbrace> \<longmapsto> B \<^bold>w\<^bold>i\<^bold>t\<^bold>h P \<^bold>w\<^bold>h\<^bold>e\<^bold>n Q"
+  "\<^bold>c\<^bold>a\<^bold>s\<^bold>t A \<longmapsto> x \<tycolon> X \<^bold>w\<^bold>i\<^bold>t\<^bold>h P \<^bold>w\<^bold>h\<^bold>e\<^bold>n Q" == "\<^bold>c\<^bold>a\<^bold>s\<^bold>t A \<longmapsto> \<tort_lbrace> x \<tycolon> X \<tort_rbrace> \<^bold>w\<^bold>i\<^bold>t\<^bold>h P \<^bold>w\<^bold>h\<^bold>e\<^bold>n Q"
+  "\<^bold>c\<^bold>a\<^bold>s\<^bold>t A \<longmapsto> x \<tycolon> X \<^bold>w\<^bold>i\<^bold>t\<^bold>h P' \<^bold>d\<^bold>u\<^bold>a\<^bold>l A' \<longmapsto> B' \<^bold>w\<^bold>h\<^bold>e\<^bold>n P" == "\<^bold>c\<^bold>a\<^bold>s\<^bold>t A \<longmapsto> \<tort_lbrace>x \<tycolon> X\<tort_rbrace> \<^bold>w\<^bold>i\<^bold>t\<^bold>h P' \<^bold>d\<^bold>u\<^bold>a\<^bold>l A' \<longmapsto> B' \<^bold>w\<^bold>h\<^bold>e\<^bold>n P"
+  "\<^bold>c\<^bold>a\<^bold>s\<^bold>t a \<tycolon> A \<longmapsto> B \<^bold>w\<^bold>i\<^bold>t\<^bold>h P' \<^bold>d\<^bold>u\<^bold>a\<^bold>l A' \<longmapsto> B' \<^bold>w\<^bold>h\<^bold>e\<^bold>n P" == "\<^bold>c\<^bold>a\<^bold>s\<^bold>t \<tort_lbrace>a \<tycolon> A\<tort_rbrace> \<longmapsto> B \<^bold>w\<^bold>i\<^bold>t\<^bold>h P' \<^bold>d\<^bold>u\<^bold>a\<^bold>l A' \<longmapsto> B' \<^bold>w\<^bold>h\<^bold>e\<^bold>n P"
+  "\<^bold>c\<^bold>a\<^bold>s\<^bold>t A \<longmapsto> B \<^bold>w\<^bold>i\<^bold>t\<^bold>h P' \<^bold>d\<^bold>u\<^bold>a\<^bold>l a' \<tycolon> A' \<longmapsto> B' \<^bold>w\<^bold>h\<^bold>e\<^bold>n P" == "\<^bold>c\<^bold>a\<^bold>s\<^bold>t A \<longmapsto> B \<^bold>w\<^bold>i\<^bold>t\<^bold>h P' \<^bold>d\<^bold>u\<^bold>a\<^bold>l \<tort_lbrace>a' \<tycolon> A'\<tort_rbrace> \<longmapsto> B' \<^bold>w\<^bold>h\<^bold>e\<^bold>n P"
+  "\<^bold>c\<^bold>a\<^bold>s\<^bold>t A \<longmapsto> B \<^bold>w\<^bold>i\<^bold>t\<^bold>h P' \<^bold>d\<^bold>u\<^bold>a\<^bold>l A' \<longmapsto> b' \<tycolon> B' \<^bold>w\<^bold>h\<^bold>e\<^bold>n P" == "\<^bold>c\<^bold>a\<^bold>s\<^bold>t A \<longmapsto> B \<^bold>w\<^bold>i\<^bold>t\<^bold>h P' \<^bold>d\<^bold>u\<^bold>a\<^bold>l A' \<longmapsto> \<tort_lbrace>b' \<tycolon> B'\<tort_rbrace> \<^bold>w\<^bold>h\<^bold>e\<^bold>n P"
+
+
+(* abbreviation SimpleCast :: " 'a set \<Rightarrow> 'a set \<Rightarrow> bool " ("(2\<^bold>c\<^bold>a\<^bold>s\<^bold>t _ \<longmapsto> _)" [2,14] 13)
+  where "(\<^bold>c\<^bold>a\<^bold>s\<^bold>t A \<longmapsto> B) \<equiv> (\<^bold>c\<^bold>a\<^bold>s\<^bold>t A \<longmapsto> B \<^bold>w\<^bold>i\<^bold>t\<^bold>h True)" *)
+(* lemma CastE[elim]: "\<^bold>c\<^bold>a\<^bold>s\<^bold>t A \<longmapsto> B \<^bold>w\<^bold>i\<^bold>t\<^bold>h P \<Longrightarrow> (\<not> Inhabited A \<Longrightarrow> C) \<Longrightarrow> (Inhabited A \<Longrightarrow> Inhabited B \<Longrightarrow> A \<subseteq> B \<Longrightarrow> P \<Longrightarrow> C) \<Longrightarrow> C"
+   unfolding Cast_def Inhabited_def by (auto intro: Inhabited_subset)
+lemma CastI[intro]: "Inhabited A \<Longrightarrow> A \<subseteq> B \<Longrightarrow> P \<Longrightarrow> \<^bold>c\<^bold>a\<^bold>s\<^bold>t A \<longmapsto> B \<^bold>w\<^bold>i\<^bold>t\<^bold>h P"
+  and [intro]: "\<not> Inhabited A \<Longrightarrow> \<^bold>c\<^bold>a\<^bold>s\<^bold>t A \<longmapsto> B \<^bold>w\<^bold>i\<^bold>t\<^bold>h P" unfolding Cast_def Inhabited_def by auto *)
+lemma cast_id[\<nu>intro0]: "\<^bold>c\<^bold>a\<^bold>s\<^bold>t A \<longmapsto> A" unfolding Cast_def by fast
+lemma cast_dual_id[\<nu>intro0]: "\<^bold>c\<^bold>a\<^bold>s\<^bold>t A \<longmapsto> A \<^bold>d\<^bold>u\<^bold>a\<^bold>l B \<longmapsto> B" unfolding CastDual_def  by (simp add: cast_id)
+
+lemma "=_\<nu>cast": "\<^bold>p\<^bold>a\<^bold>r\<^bold>a\<^bold>m x' \<Longrightarrow> \<^bold>p\<^bold>r\<^bold>e\<^bold>m\<^bold>i\<^bold>s\<^bold>e x = x' \<Longrightarrow> \<^bold>c\<^bold>a\<^bold>s\<^bold>t x \<tycolon> N \<longmapsto> x' \<tycolon> N" unfolding Cast_def by auto
+lemma [\<nu>intro']: "\<^bold>p\<^bold>r\<^bold>e\<^bold>m\<^bold>i\<^bold>s\<^bold>e N = N' \<Longrightarrow> \<^bold>p\<^bold>r\<^bold>e\<^bold>m\<^bold>i\<^bold>s\<^bold>e x = x' \<Longrightarrow> \<^bold>c\<^bold>a\<^bold>s\<^bold>t \<tort_lbrace>x \<tycolon> N\<tort_rbrace> \<longmapsto> \<tort_lbrace>x' \<tycolon> N'\<tort_rbrace>" unfolding Cast_def Premise_def by simp
+lemma [\<nu>intro0]: "\<^bold>p\<^bold>r\<^bold>e\<^bold>m\<^bold>i\<^bold>s\<^bold>e x = x" unfolding Premise_def by simp
+
+lemma cast_trans: "\<^bold>c\<^bold>a\<^bold>s\<^bold>t A \<longmapsto> B \<^bold>w\<^bold>i\<^bold>t\<^bold>h P \<Longrightarrow> \<^bold>c\<^bold>a\<^bold>s\<^bold>t B \<longmapsto> C \<^bold>w\<^bold>i\<^bold>t\<^bold>h Q \<Longrightarrow> \<^bold>c\<^bold>a\<^bold>s\<^bold>t A \<longmapsto> C \<^bold>w\<^bold>i\<^bold>t\<^bold>h P \<and> Q"
+  unfolding Cast_def by auto
+(* lemma dual_cast_fallback[\<nu>intro']: "\<^bold>c\<^bold>a\<^bold>s\<^bold>t A \<longmapsto> B \<^bold>w\<^bold>i\<^bold>t\<^bold>h P \<Longrightarrow> (\<^bold>c\<^bold>a\<^bold>s\<^bold>t A \<longmapsto> B) \<and> (\<^bold>c\<^bold>a\<^bold>s\<^bold>t C \<longmapsto> C)" unfolding Cast_def by fast *)
+
+
+section \<open>Essential \<nu>-abstractor\<close>
+
+subsection \<open>Separation Conjecture\<close>
+
+definition disjoint :: " 'a set \<Rightarrow> 'a set \<Rightarrow> bool " (infixl "\<perpendicular>" 60) where "disjoint A B \<longleftrightarrow> (A \<inter> B = {})"
+lemma disjoint_rewL: "A \<perpendicular> B \<longleftrightarrow> (\<forall>x. x \<in> A \<longrightarrow> x \<notin> B)" unfolding disjoint_def by auto
+lemma disjoint_rewR: "A \<perpendicular> B \<longleftrightarrow> (\<forall>x. x \<in> B \<longrightarrow> x \<notin> A)" unfolding disjoint_def by auto
+
+lemma [iff]: "{} \<perpendicular> S" and [iff]: "S \<perpendicular> {}" unfolding disjoint_def by auto
+
+definition Separation :: " (heap, 'a) \<nu> \<Rightarrow> (heap, 'b) \<nu> \<Rightarrow> (heap, 'a \<times> 'b) \<nu>" (infixr "\<^emph>" 70)
+  where "A \<^emph> B = (\<lambda>h (a,b). (\<exists>h1 h2. h = h1 ++ h2 \<and> dom h1 \<perpendicular> dom h2 \<and> (h1 \<nuLinkL> A \<nuLinkR> a) \<and> (h2 \<nuLinkL> B \<nuLinkR> b)))"
+
+lemma [iff]: "h \<nuLinkL> A \<^emph> B \<nuLinkR> (a,b) \<longleftrightarrow>
+  (\<exists>h1 h2. h = h1 ++ h2 \<and> dom h1 \<perpendicular> dom h2 \<and> (h1 \<nuLinkL> A \<nuLinkR> a) \<and> (h2 \<nuLinkL> B \<nuLinkR> b))"
+  unfolding Separation_def Refining_ex by simp
+
+definition Heap_Delimiter :: "(heap,'ax) \<nu> \<Rightarrow> (heap,'bx) \<nu> \<Rightarrow> (heap, 'ax \<times> 'bx) \<nu>" (infixr "<heap-sep>" 70)
+  where "A <heap-sep> B = A \<^emph> B"
+abbreviation Heap_Delimiter_sugar :: " (heap, 'ax) typing \<Rightarrow> (heap, 'bx) typing \<Rightarrow> (heap, 'bx \<times> 'ax) typing " ( "_/ \<heavy_asterisk> _" [14,15] 14)
+  where "(A \<heavy_asterisk> B) \<equiv> (typing_img B, typing_img A) \<tycolon> (typing_nu B <heap-sep> typing_nu A)"
+
+lemma [simp]: " (a \<tycolon> A \<heavy_asterisk> b \<tycolon> B) = ((b,a) \<tycolon> (B <heap-sep> A)) " by auto
+translations " (a \<tycolon> A) \<heavy_asterisk> (b \<tycolon> B) " \<rightleftharpoons> " (CONST Pair b a) \<tycolon> (B <heap-sep> A) "
+
+lemma [cong]: "\<tort_lbrace> a \<tycolon> A \<tort_rbrace> \<equiv> \<tort_lbrace>a' \<tycolon> A'\<tort_rbrace> \<Longrightarrow> \<tort_lbrace> b \<tycolon> B \<tort_rbrace> \<equiv> \<tort_lbrace>b' \<tycolon> B'\<tort_rbrace> \<Longrightarrow> \<tort_lbrace> a \<tycolon> A \<heavy_asterisk> b \<tycolon> B \<tort_rbrace> \<equiv> \<tort_lbrace> a' \<tycolon> A' \<heavy_asterisk> b' \<tycolon> B' \<tort_rbrace>"
+  unfolding atomize_eq unfolding Heap_Delimiter_def by auto
+
+
+
+
+
+(*definition Separation :: " heap set \<Rightarrow> heap set \<Rightarrow> heap set" (infixl "\<heavy_asterisk>" 14)
+  where "Separation H1 H2 = {h. (\<exists>h1 h2. h = h1 ++ h2 \<and> dom h1 \<perpendicular> dom h2 \<and> h1 \<in> H1 \<and> h2 \<in> H2) }"
+definition NonSeparation :: " heap set \<Rightarrow> heap set \<Rightarrow> heap set" (infixl "\<dbl_and>" 13)
+  where "NonSeparation H1 H2 = {h. h \<in> H1 \<and> (\<exists>h'. h' \<subseteq>\<^sub>m h \<and> h' \<in> H2)}"
+
+translations
+  "H \<heavy_asterisk> x \<tycolon> T" == "H \<heavy_asterisk> \<tort_lbrace> x \<tycolon> T \<tort_rbrace>"
+  "x \<tycolon> T \<heavy_asterisk> H" == "\<tort_lbrace> x \<tycolon> T \<tort_rbrace> \<heavy_asterisk> H"
+  "H \<dbl_and> x \<tycolon> T" == "H \<dbl_and> \<tort_lbrace> x \<tycolon> T \<tort_rbrace>"
+  "x \<tycolon> T \<dbl_and> H" == "\<tort_lbrace> x \<tycolon> T \<tort_rbrace> \<dbl_and> H"
+
+lemma [iff]: "h \<in> (H1 \<heavy_asterisk> H2) \<longleftrightarrow> (\<exists>h1 h2. h = h1 ++ h2 \<and> dom h1 \<perpendicular> dom h2 \<and> h1 \<in> H1 \<and> h2 \<in> H2)" unfolding Separation_def by simp
+lemma [iff]: "h \<in> (H1 \<dbl_and> H2) \<longleftrightarrow> (h \<in> H1 \<and> (\<exists>h'. h' \<subseteq>\<^sub>m h \<and> h' \<in> H2))" unfolding NonSeparation_def by simp
+*)
+
+lemma [simp]: "A \<inter> S \<perpendicular> A \<inter> -S"
+  unfolding disjoint_def by auto
+lemma heap_split_id: "P h1' h2' \<Longrightarrow> \<exists>h1 h2. h1' ++ h2' = h1 ++ h2 \<and> P h1 h2" by auto
+lemma heap_split_by_set: "P (h |` S) (h |` (- S)) \<Longrightarrow> \<exists>h1 h2. h = h1 ++ h2 \<and> dom h1 \<perpendicular> dom h2 \<and> P h1 h2"
+  by (rule exI[of _ "h |` S"], rule exI[of _ "h |` (- S)"])
+    (auto simp add: map_add_def option.case_eq_if restrict_map_def disjoint_def disjoint_iff domIff)
+lemma heap_split_by_addr_set: "P (h |` (MemAddress ` S)) (h |` (- (MemAddress ` S))) \<Longrightarrow> \<exists>h1 h2. h = h1 ++ h2 \<and> dom h1 \<perpendicular> dom h2 \<and> P h1 h2"
+  using heap_split_by_set .
+
+lemma Separation_comm: " \<tort_lbrace> a \<tycolon> A \<heavy_asterisk> b \<tycolon> B\<tort_rbrace> = \<tort_lbrace>b \<tycolon> B \<heavy_asterisk> a \<tycolon> A\<tort_rbrace>" unfolding Heap_Delimiter_def
+  by (auto 4 4 simp add: disjoint_def inf_commute dest: map_add_comm )
+ 
+lemma Separation_assoc: "\<tort_lbrace> a \<tycolon> A \<heavy_asterisk> (b \<tycolon> B \<heavy_asterisk> c \<tycolon> C)\<tort_rbrace> = \<tort_lbrace>a \<tycolon> A \<heavy_asterisk> b \<tycolon> B \<heavy_asterisk> c \<tycolon> C\<tort_rbrace>"
+  unfolding Heap_Delimiter_def
+  by (auto simp add: disjoint_def) 
+    (metis (no_types, lifting) Un_empty dom_map_add inf_sup_distrib1 inf_sup_distrib2 map_add_assoc)+
+
+(* lemma NonSeparation_distrib_L: "h \<in> (A \<heavy_asterisk> (B \<dbl_and> P)) \<Longrightarrow> h \<in> (A \<heavy_asterisk> B \<dbl_and> P)"
+  using map_le_map_add map_le_trans by blast
+lemma NonSeparation_distrib_R: "h \<in> ((A \<dbl_and> P) \<heavy_asterisk> B) \<Longrightarrow> h \<in> (A \<heavy_asterisk> B \<dbl_and> P)"
+  by (metis NonSeparation_distrib_L Separation_comm) *)
+  
+
+lemma [elim!,\<nu>elim]: "Inhabited \<tort_lbrace> a \<tycolon> A \<heavy_asterisk> b \<tycolon> B \<tort_rbrace> \<Longrightarrow> (a \<ratio> A \<Longrightarrow> b \<ratio> B \<Longrightarrow> C) \<Longrightarrow> C"
+  unfolding Inhabited_def Heap_Delimiter_def by auto
+(* lemma [elim!,\<nu>elim]: "Inhabited (A \<dbl_and> B) \<Longrightarrow> (Inhabited A \<Longrightarrow> Inhabited B \<Longrightarrow> C) \<Longrightarrow> C"
+  unfolding Inhabited_def by auto *)
+
+subsubsection \<open>Fusion and Stack Delimiter operator\<close>
+
+definition Fusion :: "('a1::lrep,'b1) \<nu> \<Rightarrow> ('a2::lrep,'b2) \<nu> \<Rightarrow> ('a1 \<times> 'a2, 'b1 \<times> 'b2) \<nu>" (infixr "\<cross_product>" 70) 
+  where "Fusion N M p x = (case p of (p1,p2) \<Rightarrow> case x of (x1,x2) \<Rightarrow> (p1 \<nuLinkL> N \<nuLinkR> x1) \<and> (p2 \<nuLinkL> M \<nuLinkR> x2))"
+
+lemma [simp]: "(p1,p2) \<nuLinkL> N \<cross_product> M \<nuLinkR> (x1,x2) \<longleftrightarrow> (p1 \<nuLinkL> N \<nuLinkR> x1) \<and> (p2 \<nuLinkL> M \<nuLinkR> x2)"
+  by (simp add: Fusion_def Refining_ex)
+lemma [elim,\<nu>elim]: "(x1,x2) \<ratio> N1 \<cross_product> N2 \<Longrightarrow> (x1 \<ratio> N1 \<Longrightarrow> x2 \<ratio> N2 \<Longrightarrow> C) \<Longrightarrow> C" unfolding Inhabited_def by auto
+
+lemma [\<nu>intro]: "\<nu>Zero N z1 \<Longrightarrow> \<nu>Zero M z2 \<Longrightarrow> \<nu>Zero (N \<cross_product> M) (z1,z2)" unfolding \<nu>Zero_def by simp
+
+lemma [\<nu>intro]: "\<^bold>c\<^bold>a\<^bold>s\<^bold>t x \<tycolon> N \<longmapsto> x' \<tycolon> N' \<^bold>w\<^bold>i\<^bold>t\<^bold>h P \<Longrightarrow> \<^bold>c\<^bold>a\<^bold>s\<^bold>t y \<tycolon> M \<longmapsto> y' \<tycolon> M' \<^bold>w\<^bold>i\<^bold>t\<^bold>h Q \<Longrightarrow>
+  \<^bold>c\<^bold>a\<^bold>s\<^bold>t (x,y) \<tycolon> N \<cross_product> M \<longmapsto> (x',y') \<tycolon> N' \<cross_product> M' \<^bold>w\<^bold>i\<^bold>t\<^bold>h P \<and> Q" unfolding Cast_def by auto
+
+definition Stack_Delimiter :: "('a::lrep,'ax) \<nu> \<Rightarrow> ('b::lrep,'bx) \<nu> \<Rightarrow> ('a \<times> 'b, 'ax \<times> 'bx) \<nu>" (infixr "<stack-div>" 70)
+  where "A <stack-div> B = A \<cross_product> B"
+abbreviation Stack_Delimiter_sugar :: " ('a :: stack, 'ax) typing \<Rightarrow> ('b :: lrep, 'bx) typing \<Rightarrow> ('b \<times> 'a, 'bx \<times> 'ax) typing " ( "_/ \<heavy_comma> _" [14,15] 14)
+  where "(A \<heavy_comma> B) \<equiv> (typing_img B, typing_img A) \<tycolon> (typing_nu B <stack-div> typing_nu A)"
+
+lemma [simp]: " (a \<tycolon> A \<heavy_comma> b \<tycolon> B) = ((b,a) \<tycolon> (B <stack-div> A)) " by auto
+translations " (a \<tycolon> A) \<heavy_comma> (b \<tycolon> B) " \<rightleftharpoons> " (CONST Pair b a) \<tycolon> (B <stack-div> A) "
+
+lemma [cong]: "\<tort_lbrace> a \<tycolon> A \<tort_rbrace> \<equiv> \<tort_lbrace>a' \<tycolon> A'\<tort_rbrace> \<Longrightarrow> \<tort_lbrace> b \<tycolon> B \<tort_rbrace> \<equiv> \<tort_lbrace>b' \<tycolon> B'\<tort_rbrace> \<Longrightarrow> \<tort_lbrace> a \<tycolon> A\<heavy_comma> b \<tycolon> B \<tort_rbrace> \<equiv> \<tort_lbrace> a' \<tycolon> A' \<heavy_comma> b' \<tycolon> B' \<tort_rbrace>"
+  unfolding atomize_eq unfolding Stack_Delimiter_def by auto
+
+
+subsection \<open>Existential Nu-type\<close>
+
+definition ExNu :: " ('c \<Rightarrow> ('a,'b) \<nu>) \<Rightarrow> ('a, 'c \<Rightarrow> 'b) \<nu> "
+  where "ExNu N p x = (\<exists>c. p \<nuLinkL> N c \<nuLinkR> x c)"
+lemma [simp]: "p \<nuLinkL> ExNu N \<nuLinkR> x \<longleftrightarrow> (\<exists>c. p \<nuLinkL> N c \<nuLinkR> x c)" unfolding ExNu_def Refining_ex by simp
+
+abbreviation ExNu_sugar :: " ('c \<Rightarrow> ('a,'b) typing) \<Rightarrow> ('a, 'c \<Rightarrow> 'b) typing " (binder "\<exists>* " 10)
+  where "ExNu_sugar P \<equiv> (\<lambda>c. typing_img (P c)) \<tycolon> ExNu (\<lambda>c. typing_nu (P c))"
+translations "\<exists>* a b. P" \<rightleftharpoons> "\<exists>* a. (\<exists>*b. P)"
+  "\<exists>* c. x \<tycolon> T" => "(\<lambda>c. x) \<tycolon> CONST ExNu (\<lambda>c. T)"
+  "\<exists>* c. x \<tycolon> T" <= "(\<lambda>c. x) \<tycolon> CONST ExNu (\<lambda>c''''''. T)" (*TODO: print translation that alpha-convert the c''''' *)
+notation ExNu_sugar (binder "\<exists>\<^sup>\<nu> " 10)
+
+
+lemma [simp]: "p \<in> \<S>  \<tort_lbrace>x \<tycolon> ExNu T\<tort_rbrace> \<longleftrightarrow> (\<exists>z. p \<in> \<S>  \<tort_lbrace> x z \<tycolon> T z\<tort_rbrace> )" by (auto 4 3)
+lemma [simp]: "p \<in> \<S_S> \<tort_lbrace>x \<tycolon> ExNu T\<tort_rbrace> \<longleftrightarrow> (\<exists>z. p \<in> \<S_S> \<tort_lbrace>x z \<tycolon> T z\<tort_rbrace>)" by (auto 4 3)
+lemma [simp]: "\<tort_lbrace>x \<tycolon> ExNu T \<heavy_comma> y \<tycolon> R\<tort_rbrace> = \<tort_lbrace>\<exists>* c. x c \<tycolon> T c \<heavy_comma> y \<tycolon> R \<tort_rbrace>" unfolding Stack_Delimiter_def by auto
+lemma [simp]: "\<tort_lbrace>y \<tycolon> L \<heavy_comma> x \<tycolon> ExNu T\<tort_rbrace> = \<tort_lbrace>\<exists>* c. y \<tycolon> L \<heavy_comma> x c \<tycolon> T c \<tort_rbrace>" unfolding Stack_Delimiter_def by auto
+lemma ExTyp_strip: "(\<^bold>c\<^bold>u\<^bold>r\<^bold>r\<^bold>e\<^bold>n\<^bold>t p \<^bold>r\<^bold>e\<^bold>s\<^bold>u\<^bold>l\<^bold>t\<^bold>s \<^bold>i\<^bold>n (x \<tycolon> ExNu T)) \<equiv> (\<exists>x. \<^bold>c\<^bold>u\<^bold>r\<^bold>r\<^bold>e\<^bold>n\<^bold>t p \<^bold>r\<^bold>e\<^bold>s\<^bold>u\<^bold>l\<^bold>t\<^bold>s \<^bold>i\<^bold>n T x)"
+  unfolding CurrentConstruction_def by auto
+
+(* definition ExTyp :: "('a \<Rightarrow> 'b set) \<Rightarrow> 'b set" (binder "\<exists>* " 10)
+  where   "ExTyp T = {x. (\<exists>z. x \<in> T z)}"
+notation ExTyp (binder "\<exists>'' " 10)
+  \<comment> \<open>which represents there exists some \<nu>-images (or rarely abstractors) subject to the typing.
+    And then the image subjecting the typing could be fixed as a local variable by the \<nu>-obtain command. \<close>
+
+lemma [simp]: "x \<in> ExTyp T \<longleftrightarrow> (\<exists>z. x \<in> T z)" unfolding ExTyp_def  by auto
+lemma [simp]: "x \<in> \<S> (ExTyp T) \<longleftrightarrow> (\<exists>z. x \<in> \<S> (T z))" by (auto 4 3)
+lemma [simp]: "x \<in> \<S_S> (ExTyp T) \<longleftrightarrow> (\<exists>z. x \<in> \<S_S> (T z))" by (auto 4 3)
+lemma [simp]: "(ExTyp A \<heavy_comma> R) = (\<exists>* x. (A x \<heavy_comma> R))" by auto
+lemma [simp]: "(S\<heavy_comma> ExTyp T) = (\<exists>* z. (S \<heavy_comma> T z))" by auto
+lemma ExTyp_strip: "(\<^bold>c\<^bold>u\<^bold>r\<^bold>r\<^bold>e\<^bold>n\<^bold>t p \<^bold>r\<^bold>e\<^bold>s\<^bold>u\<^bold>l\<^bold>t\<^bold>s \<^bold>i\<^bold>n (ExTyp T)) \<equiv> (\<exists>x. \<^bold>c\<^bold>u\<^bold>r\<^bold>r\<^bold>e\<^bold>n\<^bold>t p \<^bold>r\<^bold>e\<^bold>s\<^bold>u\<^bold>l\<^bold>t\<^bold>s \<^bold>i\<^bold>n T x)"
+  unfolding CurrentConstruction_def by auto *)
+
+
+(* definition AutoExTyp :: "('a \<Rightarrow> 'b set) \<Rightarrow> 'b set" (binder "\<exists>*''" 10)
+  where "AutoExTyp T = {x. (\<exists>z. x \<in> (T z))}"
+
+lemma [simp]: "x \<in> (AutoExTyp T) \<equiv> (\<exists>z. x \<in> T z)" unfolding AutoExTyp_def by auto
+lemma [simp]: "(R\<heavy_comma> AutoExTyp T) = (\<exists>*' x. (R\<heavy_comma> T x))" unfolding AutoExTyp_def by auto
+lemma [simp]: "(AutoExTyp T\<heavy_comma> R) = (\<exists>*' x. (T x\<heavy_comma> R))" unfolding AutoExTyp_def by auto
+lemma [simp]: "(AutoExTyp T \<flower> R) = (\<exists>*' x. (T x \<flower> R))" unfolding AutoExTyp_def BinderNameTag_def by auto
+
+lemma [simp]: "AutoExTyp T = (\<exists>*' a b. T (a,b))" unfolding AutoExTyp_def by auto
+
+lemma AutoExTyp_strip: "(\<^bold>c\<^bold>u\<^bold>r\<^bold>r\<^bold>e\<^bold>n\<^bold>t p \<^bold>r\<^bold>e\<^bold>s\<^bold>u\<^bold>l\<^bold>t\<^bold>s \<^bold>i\<^bold>n (AutoExTyp T)) \<equiv> (\<exists>x. \<^bold>c\<^bold>u\<^bold>r\<^bold>r\<^bold>e\<^bold>n\<^bold>t p \<^bold>r\<^bold>e\<^bold>s\<^bold>u\<^bold>l\<^bold>t\<^bold>s \<^bold>i\<^bold>n T x)"
+  unfolding AutoExTyp_def CurrentConstruction_def by (rule eq_reflection) auto *)
+
+subsection \<open>Addition Nu-type : coheres true proposition\<close>
+
+definition AddtionTy :: " 'a set \<Rightarrow> bool \<Rightarrow> 'a set " (infixl "\<addition>" 50)
+  where " (T \<addition> P) = {x. x \<in> T \<and> P}"
+lemma [simp]: "T \<addition> True = T" unfolding AddtionTy_def by simp
+lemma [simp]: "x \<in> (T \<addition> P) \<longleftrightarrow> x \<in> T \<and> P" unfolding AddtionTy_def by simp
+(* lemma [intro]: "P \<Longrightarrow> [h] x \<in>\<^sub>\<nu> T \<Longrightarrow> [h] x \<in>\<^sub>\<nu> (T \<addition> P)" by simp
+lemma [elim]: "[h] x \<in>\<^sub>\<nu> (T \<addition> P) \<Longrightarrow> ([h] x \<in>\<^sub>\<nu> T \<Longrightarrow> P \<Longrightarrow> C) \<Longrightarrow> C" by simp*)
+lemma [simp]: "(R \<heavy_comma> T \<addition> P) = ((R \<heavy_comma> T) \<addition> P)" by auto
+lemma t1: "(\<^bold>c\<^bold>u\<^bold>r\<^bold>r\<^bold>e\<^bold>n\<^bold>t s \<^bold>r\<^bold>e\<^bold>s\<^bold>u\<^bold>l\<^bold>t\<^bold>s \<^bold>i\<^bold>n T \<addition> P) \<longleftrightarrow> (\<^bold>c\<^bold>u\<^bold>r\<^bold>r\<^bold>e\<^bold>n\<^bold>t s \<^bold>r\<^bold>e\<^bold>s\<^bold>u\<^bold>l\<^bold>t\<^bold>s \<^bold>i\<^bold>n T) \<and> P" unfolding CurrentConstruction_def by (cases s) auto
+lemma [simp]: "((((\<^bold>c\<^bold>u\<^bold>r\<^bold>r\<^bold>e\<^bold>n\<^bold>t s \<^bold>r\<^bold>e\<^bold>s\<^bold>u\<^bold>l\<^bold>t\<^bold>s \<^bold>i\<^bold>n S) \<and> B) \<and> C) \<^bold>w\<^bold>i\<^bold>t\<^bold>h \<^bold>f\<^bold>a\<^bold>c\<^bold>t\<^bold>s: PROP L) \<equiv> (((\<^bold>c\<^bold>u\<^bold>r\<^bold>r\<^bold>e\<^bold>n\<^bold>t s \<^bold>r\<^bold>e\<^bold>s\<^bold>u\<^bold>l\<^bold>t\<^bold>s \<^bold>i\<^bold>n S) \<and> (B \<and> C)) \<^bold>w\<^bold>i\<^bold>t\<^bold>h \<^bold>f\<^bold>a\<^bold>c\<^bold>t\<^bold>s: PROP L)" by simp
+
+lemma move_fact_to_star1[simp]:
+  "((\<^bold>c\<^bold>u\<^bold>r\<^bold>r\<^bold>e\<^bold>n\<^bold>t s \<^bold>r\<^bold>e\<^bold>s\<^bold>u\<^bold>l\<^bold>t\<^bold>s \<^bold>i\<^bold>n S \<addition> Q) \<^bold>w\<^bold>i\<^bold>t\<^bold>h \<^bold>f\<^bold>a\<^bold>c\<^bold>t\<^bold>s: PROP FactCollection (PROP NoFact) (PROP L) (PROP I))
+    \<Longrightarrow> (\<^bold>c\<^bold>u\<^bold>r\<^bold>r\<^bold>e\<^bold>n\<^bold>t s \<^bold>r\<^bold>e\<^bold>s\<^bold>u\<^bold>l\<^bold>t\<^bold>s \<^bold>i\<^bold>n S \<^bold>w\<^bold>i\<^bold>t\<^bold>h \<^bold>f\<^bold>a\<^bold>c\<^bold>t\<^bold>s: PROP FactCollection (Trueprop Q) (PROP L) (PROP I))"
+  unfolding t1 SpecTop_imp conj_imp FactCollection_imp
+  by (intro equal_intr_rule SpecTop_I FactCollection_I conjI NoFact) (* (unfold SpecTop_imp conj_imp FactCollection_imp) *)
+lemma move_fact_to_star2[simp]:
+  "((\<^bold>c\<^bold>u\<^bold>r\<^bold>r\<^bold>e\<^bold>n\<^bold>t s \<^bold>r\<^bold>e\<^bold>s\<^bold>u\<^bold>l\<^bold>t\<^bold>s \<^bold>i\<^bold>n S \<addition> Q) \<^bold>w\<^bold>i\<^bold>t\<^bold>h \<^bold>f\<^bold>a\<^bold>c\<^bold>t\<^bold>s: PROP FactCollection (Trueprop P) (PROP L) (PROP I))
+    \<Longrightarrow> (\<^bold>c\<^bold>u\<^bold>r\<^bold>r\<^bold>e\<^bold>n\<^bold>t s \<^bold>r\<^bold>e\<^bold>s\<^bold>u\<^bold>l\<^bold>t\<^bold>s \<^bold>i\<^bold>n S \<^bold>w\<^bold>i\<^bold>t\<^bold>h \<^bold>f\<^bold>a\<^bold>c\<^bold>t\<^bold>s: PROP FactCollection  (Trueprop (Q \<and> P)) (PROP L) (PROP I))"
+  unfolding t1 SpecTop_imp conj_imp FactCollection_imp
+  by (intro equal_intr_rule SpecTop_I FactCollection_I conjI) (* (unfold SpecTop_imp conj_imp FactCollection_imp) *)
+
+
 section \<open>Syntax\<close>
 
 subsection \<open>Logical image models\<close>
@@ -86,7 +311,7 @@ parse_ast_translation \<open>[
   (\<^const_syntax>\<open>Arg_Ret_Pair_sugar\<close>, K tr_arg_ret_pair)
 ]\<close>
 
-section \<open>Mechanisms\<close>
+section \<open>Mechanisms - II\<close>
 
 
 
@@ -97,7 +322,66 @@ term "Map.empty"
 lemma Separation_emptyL: "(Nothing \<heavy_asterisk> S) = S" and Separation_emptyR: "(S \<heavy_asterisk> Nothing) = S"
   unfolding Nothing_def Separation_def by auto
 
-subsection \<open>Cast\<close>
+subsubsection \<open>Syntax & Auxiliary\<close>
+
+consts ResourceState :: " heap \<Rightarrow> 'a \<Rightarrow> 'b set \<Rightarrow> bool" ("_ \<^bold>a\<^bold>t _ \<^bold>i\<^bold>s _ " [16,16,12] 11)
+consts allocated :: " heap \<Rightarrow> 'a \<Rightarrow> bool"
+
+translations "h \<^bold>a\<^bold>t resource \<^bold>i\<^bold>s x \<tycolon> T" \<rightleftharpoons> "h \<^bold>a\<^bold>t resource \<^bold>i\<^bold>s \<tort_lbrace> x \<tycolon> T \<tort_rbrace>"
+
+definition "addr_allocated heap addr \<longleftrightarrow> MemAddress addr \<in> dom heap"
+adhoc_overloading allocated addr_allocated
+
+(* lemma addr_allocated_mono[dest]: "h \<subseteq>\<^sub>m h' \<Longrightarrow> addr_allocated h addr \<Longrightarrow> addr_allocated h' addr"
+  unfolding addr_allocated_def by auto
+lemma [iff]: "addr_allocated (h(k \<mapsto> v)) addr \<longleftrightarrow> k = MemAddress addr \<or> addr_allocated h addr"
+  and [iff]: "addr_allocated (h(k := None)) addr \<longleftrightarrow> k \<noteq> MemAddress addr \<and> addr_allocated h addr"
+  unfolding addr_allocated_def by auto *)
+lemma [iff]: "addr_allocated (h(k \<mapsto> v)) addr \<longleftrightarrow> k = MemAddress addr \<or> addr_allocated h addr"
+  and [iff]: "addr_allocated (h(k := None)) addr \<longleftrightarrow> k \<noteq> MemAddress addr \<and> addr_allocated h addr"
+  unfolding addr_allocated_def by auto
+
+definition MemAddrState :: "heap \<Rightarrow> nat memaddr \<Rightarrow> 'b::lrep set \<Rightarrow> bool"
+  where "MemAddrState h addr S \<longleftrightarrow> addr_allocated h addr \<and> shallowize (the (h (MemAddress addr))) \<in> S"
+adhoc_overloading ResourceState MemAddrState
+
+(*lemma MemAddrState_mono[dest]: "h \<subseteq>\<^sub>m h' \<Longrightarrow> MemAddrState h addr S \<Longrightarrow> MemAddrState h' addr S"
+  unfolding MemAddrState_def addr_allocated_def by auto (metis \<nu>set_mono domI map_le_def option.sel) *)
+
+lemma MemAddrState_I_neq[intro]: "k2 \<noteq> k \<Longrightarrow> MemAddrState h k2 S \<Longrightarrow> MemAddrState (h(MemAddress k := v)) k2 S"
+  and MemAddrState_I_eq[intro]: "v' \<in> S \<Longrightarrow> MemAddrState (h(MemAddress k \<mapsto> deepize v')) k S"
+  unfolding MemAddrState_def addr_allocated_def by auto
+
+lemma MemAddrState_E[elim]:
+  "MemAddrState h addr S \<Longrightarrow> (addr_allocated h addr \<Longrightarrow> Inhabited S \<Longrightarrow> C) \<Longrightarrow> C"
+  unfolding MemAddrState_def by auto
+lemma MemAddrState_I:
+  "addr_allocated h addr \<Longrightarrow> shallowize (the (h (MemAddress addr))) \<in> S \<Longrightarrow> MemAddrState h addr S"
+  unfolding MemAddrState_def by auto
+
+(* lemma MemAddrState_retained_N[intro]:
+  "k \<noteq> MemAddress addr \<Longrightarrow> MemAddrState h addr S \<Longrightarrow> \<nu>Independent S claim
+    \<Longrightarrow> Alive k \<in> claim \<Longrightarrow> MemAddrState (h(k:=None)) addr S"
+  unfolding MemAddrState_def \<nu>Independent_def by auto
+lemma MemAddrState_retained_S[intro]:
+  "k \<noteq> MemAddress addr \<Longrightarrow> MemAddrState h addr S \<Longrightarrow> \<nu>Independent S claim
+    \<Longrightarrow> Write k \<in> claim \<Longrightarrow> MemAddrState (h(k \<mapsto> v)) addr S"
+  unfolding MemAddrState_def \<nu>Independent_def by auto
+
+*)
+
+
+lemma MemAddrState_restrict_I1[intro]: "h \<^bold>a\<^bold>t a \<^bold>i\<^bold>s T \<Longrightarrow> a \<in> S \<Longrightarrow> h |` (MemAddress ` S) \<^bold>a\<^bold>t a \<^bold>i\<^bold>s T "
+  and MemAddrState_restrict_I2[intro]: "h \<^bold>a\<^bold>t a \<^bold>i\<^bold>s T \<Longrightarrow> a \<notin> S \<Longrightarrow> h |` (- MemAddress ` S) \<^bold>a\<^bold>t a \<^bold>i\<^bold>s T "
+  unfolding MemAddrState_def addr_allocated_def
+  by auto (metis ComplI imageE option.sel resource_key.inject(1) restrict_map_def)
+
+lemma MemAddrState_add_I1[intro]: " h1 \<^bold>a\<^bold>t a \<^bold>i\<^bold>s T \<Longrightarrow> dom h1 \<perpendicular> dom h2 \<Longrightarrow> h1 ++ h2 \<^bold>a\<^bold>t a \<^bold>i\<^bold>s T "
+  and  MemAddrState_add_I2[intro]: " h2 \<^bold>a\<^bold>t a \<^bold>i\<^bold>s T \<Longrightarrow> dom h1 \<perpendicular> dom h2 \<Longrightarrow> h1 ++ h2 \<^bold>a\<^bold>t a \<^bold>i\<^bold>s T "
+  unfolding MemAddrState_def addr_allocated_def by (auto simp add: map_add_def disjoint_def split: option.split)
+
+
+subsubsection \<open>Cast\<close>
 
 definition Heap_Cast_Goal :: " heap set \<Rightarrow> heap set " ("\<medium_left_bracket> _ \<medium_right_bracket>") where "Heap_Cast_Goal x = x"
   \<comment> \<open>The protector marks the goal to be gained\<close>
@@ -114,9 +398,6 @@ lemma context_cast_dual[\<nu>intro]:
     \<Longrightarrow> \<^bold>c\<^bold>a\<^bold>s\<^bold>t H \<longmapsto> \<medium_left_bracket> H' \<medium_right_bracket> \<^bold>w\<^bold>i\<^bold>t\<^bold>h PH \<^bold>d\<^bold>u\<^bold>a\<^bold>l \<medium_left_bracket> H2 \<medium_right_bracket> \<longmapsto> H2' \<^bold>w\<^bold>h\<^bold>e\<^bold>n QH
     \<Longrightarrow> \<^bold>c\<^bold>a\<^bold>s\<^bold>t (K\<heavy_comma> \<^bold>h\<^bold>e\<^bold>a\<^bold>p H) \<longmapsto> (K'\<heavy_comma> \<^bold>h\<^bold>e\<^bold>a\<^bold>p H') \<^bold>w\<^bold>i\<^bold>t\<^bold>h PK \<and> PH \<^bold>d\<^bold>u\<^bold>a\<^bold>l (K2\<heavy_comma> \<^bold>h\<^bold>e\<^bold>a\<^bold>p H2) \<longmapsto> (K2\<heavy_comma> \<^bold>h\<^bold>e\<^bold>a\<^bold>p H2') \<^bold>w\<^bold>h\<^bold>e\<^bold>n QH"
   unfolding CastDual_def Cast_def Heap_Cast_Goal_def by (auto simp add: pair_forall)
-
-
-subsubsection \<open>Separation Cast\<close>
 
 (* lemma [\<nu>intro0]: "\<^bold>c\<^bold>a\<^bold>s\<^bold>t x \<tycolon> X \<longmapsto> H' \<heavy_asterisk> y \<tycolon> Y \<^bold>w\<^bold>i\<^bold>t\<^bold>h P \<^bold>d\<^bold>u\<^bold>a\<^bold>l H'\<^sub>m \<heavy_asterisk> y\<^sub>m \<tycolon> Y \<longmapsto> x\<^sub>m \<tycolon> X \<^bold>w\<^bold>h\<^bold>e\<^bold>n Q
   \<Longrightarrow> \<^bold>c\<^bold>a\<^bold>s\<^bold>t x \<tycolon> X \<longmapsto> H' \<heavy_asterisk> \<medium_left_bracket> y \<tycolon> Y \<medium_right_bracket> \<^bold>w\<^bold>i\<^bold>t\<^bold>h P \<^bold>d\<^bold>u\<^bold>a\<^bold>l H'\<^sub>m \<heavy_asterisk> \<medium_left_bracket> y\<^sub>m \<tycolon> Y \<medium_right_bracket> \<longmapsto> x\<^sub>m \<tycolon> X \<^bold>w\<^bold>h\<^bold>e\<^bold>n Q"
@@ -191,6 +472,73 @@ lemma [\<nu>intro]: "\<^bold>c\<^bold>a\<^bold>s\<^bold>t A \<longmapsto> A' \<^
   unfolding Cast_def by auto
 lemma StackDelimiter_to_AndTy: " (A\<heavy_comma> B) \<equiv> (B \<^bold>a\<^bold>n\<^bold>d A) " unfolding Stack_Delimiter_def AndTy_def by simp
 *)
+
+subsection \<open>Cast\<close>
+
+theorem apply_cast: "(\<^bold>c\<^bold>u\<^bold>r\<^bold>r\<^bold>e\<^bold>n\<^bold>t blk \<^bold>r\<^bold>e\<^bold>s\<^bold>u\<^bold>l\<^bold>t\<^bold>s \<^bold>i\<^bold>n (R \<heavy_comma> X\<heavy_comma> \<^bold>h\<^bold>e\<^bold>a\<^bold>p H)) \<Longrightarrow> (\<^bold>c\<^bold>a\<^bold>s\<^bold>t X \<longmapsto> Y \<^bold>w\<^bold>i\<^bold>t\<^bold>h P) \<Longrightarrow> (\<^bold>c\<^bold>u\<^bold>r\<^bold>r\<^bold>e\<^bold>n\<^bold>t blk \<^bold>r\<^bold>e\<^bold>s\<^bold>u\<^bold>l\<^bold>t\<^bold>s \<^bold>i\<^bold>n (R \<heavy_comma> Y\<heavy_comma> \<^bold>h\<^bold>e\<^bold>a\<^bold>p H) \<addition> P)"
+  unfolding Procedure_def CurrentConstruction_def PendingConstruction_def bind_def SpecTop_imp Cast_def by (auto 4 6)
+theorem "cast": "\<^bold>c\<^bold>u\<^bold>r\<^bold>r\<^bold>e\<^bold>n\<^bold>t blk \<^bold>r\<^bold>e\<^bold>s\<^bold>u\<^bold>l\<^bold>t\<^bold>s \<^bold>i\<^bold>n T \<Longrightarrow> \<^bold>c\<^bold>a\<^bold>s\<^bold>t T \<longmapsto> T' \<^bold>w\<^bold>i\<^bold>t\<^bold>h P \<^bold>w\<^bold>h\<^bold>e\<^bold>n Q \<Longrightarrow> \<^bold>p\<^bold>r\<^bold>e\<^bold>m\<^bold>i\<^bold>s\<^bold>e Q \<Longrightarrow> \<^bold>c\<^bold>u\<^bold>r\<^bold>r\<^bold>e\<^bold>n\<^bold>t blk \<^bold>r\<^bold>e\<^bold>s\<^bold>u\<^bold>l\<^bold>t\<^bold>s \<^bold>i\<^bold>n T' "
+  for T' :: "(heap \<times> 'a::lrep) set" unfolding Cast_def CurrentConstruction_def by auto
+
+(* theorem proc_cast': "\<^bold>p\<^bold>r\<^bold>o\<^bold>c f \<blangle> A \<longmapsto> B \<brangle> \<Longrightarrow> \<^bold>c\<^bold>a\<^bold>s\<^bold>t A' \<longmapsto> A \<^bold>w\<^bold>i\<^bold>t\<^bold>h P \<Longrightarrow> \<^bold>c\<^bold>a\<^bold>s\<^bold>t B \<longmapsto> B' \<^bold>w\<^bold>i\<^bold>t\<^bold>h Q \<Longrightarrow> \<^bold>p\<^bold>r\<^bold>o\<^bold>c f \<blangle> A' \<longmapsto> B' \<brangle>"
+  unfolding Procedure_def Cast_def by (auto 0 4) *)
+
+lemma [\<nu>intro']: "\<^bold>i\<^bold>n\<^bold>t\<^bold>r\<^bold>o \<^bold>c\<^bold>a\<^bold>s\<^bold>t A \<longmapsto> B \<^bold>w\<^bold>i\<^bold>t\<^bold>h P \<Longrightarrow> \<^bold>c\<^bold>a\<^bold>s\<^bold>t A \<longmapsto> B \<^bold>w\<^bold>i\<^bold>t\<^bold>h P" unfolding Intro_def .
+lemma [\<nu>intro']: "\<^bold>d\<^bold>e\<^bold>s\<^bold>t \<^bold>c\<^bold>a\<^bold>s\<^bold>t A \<longmapsto> B \<^bold>w\<^bold>i\<^bold>t\<^bold>h P \<Longrightarrow> \<^bold>c\<^bold>a\<^bold>s\<^bold>t A \<longmapsto> B \<^bold>w\<^bold>i\<^bold>t\<^bold>h P" unfolding Dest_def .
+
+lemma "\<^bold>i\<^bold>n\<^bold>t\<^bold>r\<^bold>o \<^bold>c\<^bold>a\<^bold>s\<^bold>t A \<longmapsto> A" unfolding Intro_def using cast_id .
+lemma "\<^bold>d\<^bold>e\<^bold>s\<^bold>t \<^bold>c\<^bold>a\<^bold>s\<^bold>t A \<longmapsto> A" unfolding Dest_def using cast_id .
+  \<comment> \<open>All intro-cast or dest-cast involved in the reasoner constitute a directed acyclic graph WITH self-loop.
+    Note the self-loop has the lowest priority, so that the self-loop only be tried ONCE in the whole reasoning
+      (when all other rules cannot be applied), and only longest inference chains (who cannot be extended by
+      any other rules) will be tried by self-loop.
+    \<^term>\<open>Different\<close> can be used to assert the non-self-loop.\<close>
+
+subsection \<open>Conversion\<close>
+
+(* definition AutoTag :: "bool \<Rightarrow> bool" ("\<^bold>a\<^bold>u\<^bold>t\<^bold>o _" [100] 99) where [\<nu>def]: "\<^bold>a\<^bold>u\<^bold>t\<^bold>o P \<longleftrightarrow> P"
+lemma [\<nu>intro]: "[heap] \<^bold>c\<^bold>a\<^bold>s\<^bold>t U \<longmapsto> U' \<Longrightarrow> \<^bold>a\<^bold>u\<^bold>t\<^bold>o \<^bold>p\<^bold>r\<^bold>o\<^bold>c nop \<blangle> U \<longmapsto> U' \<brangle>"
+  unfolding AutoTag_def Cast_def Procedure_def nop_def by auto *)
+  
+definition Conversion :: "('a::lrep \<longmapsto> 'b::lrep) \<Rightarrow> (heap\<times>'a) set \<Rightarrow> (heap\<times>'b) set \<Rightarrow> ( ('c::lrep) \<longmapsto> ('d::lrep)) \<Rightarrow> (heap\<times>'c) set \<Rightarrow> (heap\<times>'d) set \<Rightarrow> bool"
+    ("\<^bold>c\<^bold>o\<^bold>n\<^bold>v\<^bold>e\<^bold>r\<^bold>s\<^bold>i\<^bold>o\<^bold>n _/ (2\<blangle> _/ \<longmapsto> _ \<brangle>)/ \<long_dobule_mapsto> _/ (2\<blangle> _/ \<longmapsto> _ \<brangle>)" [101,2,2,101,2,2] 100)
+    where [\<nu>def]: "\<^bold>c\<^bold>o\<^bold>n\<^bold>v\<^bold>e\<^bold>r\<^bold>s\<^bold>i\<^bold>o\<^bold>n f \<blangle> U \<longmapsto> V \<brangle> \<long_dobule_mapsto> g \<blangle> U' \<longmapsto> V' \<brangle> \<longleftrightarrow>( \<^bold>p\<^bold>r\<^bold>o\<^bold>c f \<blangle> U \<longmapsto> V \<brangle> \<longrightarrow> \<^bold>p\<^bold>r\<^bold>o\<^bold>c g \<blangle> U' \<longmapsto> V' \<brangle> )"
+
+lemma conversion: "\<^bold>c\<^bold>o\<^bold>n\<^bold>v\<^bold>e\<^bold>r\<^bold>s\<^bold>i\<^bold>o\<^bold>n f \<blangle> U \<longmapsto> V \<brangle> \<long_dobule_mapsto> f' \<blangle> U' \<longmapsto> V' \<brangle> \<Longrightarrow> \<^bold>p\<^bold>r\<^bold>o\<^bold>c f \<blangle> U \<longmapsto> V \<brangle> \<Longrightarrow> \<^bold>p\<^bold>r\<^bold>o\<^bold>c f' \<blangle> U' \<longmapsto> V' \<brangle>"
+  for f :: " ('a::lrep) \<longmapsto> ('b::lrep)" and f' :: " ('c::lrep) \<longmapsto> ('d::lrep)" unfolding Conversion_def by fast
+
+lemma [\<nu>intro0]: "\<^bold>c\<^bold>o\<^bold>n\<^bold>v\<^bold>e\<^bold>r\<^bold>s\<^bold>i\<^bold>o\<^bold>n f \<blangle> U \<longmapsto> V \<brangle> \<long_dobule_mapsto> f \<blangle> U \<longmapsto> V \<brangle>" unfolding Conversion_def by fast
+
+lemma conversion_cast[\<nu>intro]: "\<^bold>c\<^bold>a\<^bold>s\<^bold>t U' \<longmapsto> U \<^bold>w\<^bold>i\<^bold>t\<^bold>h P \<^bold>d\<^bold>u\<^bold>a\<^bold>l V \<longmapsto> V' \<^bold>w\<^bold>h\<^bold>e\<^bold>n Q \<Longrightarrow> \<^bold>p\<^bold>r\<^bold>e\<^bold>m\<^bold>i\<^bold>s\<^bold>e (P \<longrightarrow> Q) \<Longrightarrow> \<^bold>c\<^bold>o\<^bold>n\<^bold>v\<^bold>e\<^bold>r\<^bold>s\<^bold>i\<^bold>o\<^bold>n f \<blangle> U \<longmapsto> V \<brangle> \<long_dobule_mapsto> f \<blangle> U' \<longmapsto> V'\<brangle>"
+  unfolding Conversion_def Procedure_def Cast_def CastDual_def id_def
+  by (metis Cast_def CurrentConstruction_def LooseStateTy_introByStrict LooseStateTy_upgrade Premise_def "cast")
+(* lemma [\<nu>intro]: "\<^bold>p\<^bold>r\<^bold>o\<^bold>c g \<blangle> U' \<longmapsto> U \<brangle> \<Longrightarrow> \<^bold>c\<^bold>o\<^bold>n\<^bold>v\<^bold>e\<^bold>r\<^bold>s\<^bold>i\<^bold>o\<^bold>n f \<blangle> U \<longmapsto> V \<brangle> \<long_dobule_mapsto> (g \<nuInstrComp> f) \<blangle> U' \<longmapsto> V\<brangle>"
+  unfolding Conversion_def using instr_comp by fast *)
+
+theorem apply_proc_conv: "(\<^bold>c\<^bold>u\<^bold>r\<^bold>r\<^bold>e\<^bold>n\<^bold>t blk \<^bold>r\<^bold>e\<^bold>s\<^bold>u\<^bold>l\<^bold>t\<^bold>s \<^bold>i\<^bold>n S) \<Longrightarrow> (\<^bold>c\<^bold>o\<^bold>n\<^bold>v\<^bold>e\<^bold>r\<^bold>s\<^bold>i\<^bold>o\<^bold>n f \<blangle> S' \<longmapsto> T' \<brangle> \<long_dobule_mapsto> g \<blangle> S \<longmapsto> T\<brangle>) \<Longrightarrow> \<^bold>p\<^bold>r\<^bold>o\<^bold>c f \<blangle> S' \<longmapsto> T' \<brangle> \<Longrightarrow> (\<^bold>p\<^bold>e\<^bold>n\<^bold>d\<^bold>i\<^bold>n\<^bold>g g \<^bold>o\<^bold>n blk \<^bold>r\<^bold>e\<^bold>s\<^bold>u\<^bold>l\<^bold>t\<^bold>s \<^bold>i\<^bold>n T)"
+  unfolding Procedure_def CurrentConstruction_def PendingConstruction_def bind_def SpecTop_imp Conversion_def by auto
+
+lemma conversion_trans: "\<^bold>c\<^bold>o\<^bold>n\<^bold>v\<^bold>e\<^bold>r\<^bold>s\<^bold>i\<^bold>o\<^bold>n g \<blangle> Xg \<longmapsto> Yg \<brangle> \<long_dobule_mapsto> h \<blangle> Xh \<longmapsto> Yh \<brangle>
+  \<Longrightarrow> \<^bold>c\<^bold>o\<^bold>n\<^bold>v\<^bold>e\<^bold>r\<^bold>s\<^bold>i\<^bold>o\<^bold>n f \<blangle> Xf \<longmapsto> Yf \<brangle> \<long_dobule_mapsto> g \<blangle> Xg \<longmapsto> Yg \<brangle>
+  \<Longrightarrow> \<^bold>c\<^bold>o\<^bold>n\<^bold>v\<^bold>e\<^bold>r\<^bold>s\<^bold>i\<^bold>o\<^bold>n f \<blangle> Xf \<longmapsto> Yf\<brangle> \<long_dobule_mapsto> h \<blangle> Xh \<longmapsto> Yh \<brangle>"
+  unfolding Conversion_def by blast
+
+
+ subsubsection \<open>Auto construct & destruct\<close>
+
+definition AutoConstruct :: " 'exp \<Rightarrow> ('a::lrep \<longmapsto> 'b::lrep) \<Rightarrow> (heap \<times> 'a) set \<Rightarrow> (heap \<times> 'b) set \<Rightarrow> bool "("\<^bold>c\<^bold>o\<^bold>n\<^bold>s\<^bold>t\<^bold>r\<^bold>u\<^bold>c\<^bold>t _/ \<^bold>b\<^bold>y \<^bold>p\<^bold>r\<^bold>o\<^bold>c _/ (2\<blangle>_/ \<longmapsto> _ \<brangle>)" [20,101,10,10] 100)
+  where [\<nu>def]:"AutoConstruct exp f S T \<longleftrightarrow> \<^bold>p\<^bold>r\<^bold>o\<^bold>c f \<blangle> S \<longmapsto> T \<brangle>"
+lemma AutoConstruct: "(\<^bold>c\<^bold>u\<^bold>r\<^bold>r\<^bold>e\<^bold>n\<^bold>t blk \<^bold>r\<^bold>e\<^bold>s\<^bold>u\<^bold>l\<^bold>t\<^bold>s \<^bold>i\<^bold>n S) \<Longrightarrow> AutoConstruct exp f S T \<Longrightarrow> (\<^bold>p\<^bold>e\<^bold>n\<^bold>d\<^bold>i\<^bold>n\<^bold>g f \<^bold>o\<^bold>n blk \<^bold>r\<^bold>e\<^bold>s\<^bold>u\<^bold>l\<^bold>t\<^bold>s \<^bold>i\<^bold>n T)" for exp :: "'exp"
+  unfolding AutoConstruct_def using apply_proc .
+
+(* lemma [simp]: "(Inhabited A \<and> Inhabited B) \<or> (Inhabited A' \<and> Inhabited B')
+  \<Longrightarrow> (A\<heavy_comma>B) = (A'\<heavy_comma>B') \<longleftrightarrow> A = A' \<and> B = B'" unfolding Stack_Delimiter_def Inhabited_def by (auto simp add: times_eq_iff) 
+lemma  [elim]: "(A\<heavy_comma>B) = (A'\<heavy_comma>B') \<Longrightarrow> (A = {} \<or> B = {} \<Longrightarrow> A' = {} \<or> B' = {} \<Longrightarrow> C) \<Longrightarrow> (A = A' \<Longrightarrow> B = B' \<Longrightarrow> C) \<Longrightarrow> C"
+  unfolding Stack_Delimiter_def by (auto simp add: times_eq_iff)
+*)
+
+
+
 subsection \<open>Index for Shallow Representation\<close>
 
 text \<open>Indexes provide the function to access and map the addressed part in a nested structure (e.g. a nested pair @{term "(a,((b,c),d))"}.
@@ -322,16 +670,16 @@ definition op_depair :: "(('b::lrep) \<times> ('a::lrep)) \<times> ('r::stack) \
   where "op_depair h x = (case x of ((b,a),r) \<Rightarrow> Success h (a,b,r))"
 (* declare op_pair_def[\<nu>instr] op_depair_def[\<nu>instr] *)
 
-theorem pr_\<nu>proc: "\<^bold>p\<^bold>r\<^bold>o\<^bold>c op_pair \<blangle> R \<heavy_comma> a \<tycolon> A \<heavy_comma> b \<tycolon> B \<longmapsto> R \<heavy_comma> (a,b) \<tycolon> (A \<nuFusion> B) \<brangle>" unfolding \<nu>def  op_pair_def by auto
-theorem dpr_\<nu>proc: "\<^bold>p\<^bold>r\<^bold>o\<^bold>c op_depair \<blangle> R \<heavy_comma> (a,b) \<tycolon> (A \<nuFusion> B) \<longmapsto> R \<heavy_comma> a \<tycolon> A \<heavy_comma> b \<tycolon> B \<brangle>" unfolding \<nu>def  op_depair_def by auto
+theorem pr_\<nu>proc: "\<^bold>p\<^bold>r\<^bold>o\<^bold>c op_pair \<blangle> R \<heavy_comma> a \<tycolon> A \<heavy_comma> b \<tycolon> B \<longmapsto> R \<heavy_comma> (a,b) \<tycolon> (A \<cross_product> B) \<brangle>" unfolding \<nu>def  op_pair_def by auto
+theorem dpr_\<nu>proc: "\<^bold>p\<^bold>r\<^bold>o\<^bold>c op_depair \<blangle> R \<heavy_comma> (a,b) \<tycolon> (A \<cross_product> B) \<longmapsto> R \<heavy_comma> a \<tycolon> A \<heavy_comma> b \<tycolon> B \<brangle>" unfolding \<nu>def  op_depair_def by auto
 (*
-lemma pr_auto_schema: "\<^bold>p\<^bold>r\<^bold>o\<^bold>c call op_pair \<blangle> R \<heavy_comma> a \<tycolon> A \<heavy_comma> b \<tycolon> B \<flower> W \<longmapsto> R \<heavy_comma> (a,b) \<tycolon> (A \<nuFusion>' B) \<flower> W \<brangle>"
+lemma pr_auto_schema: "\<^bold>p\<^bold>r\<^bold>o\<^bold>c call op_pair \<blangle> R \<heavy_comma> a \<tycolon> A \<heavy_comma> b \<tycolon> B \<flower> W \<longmapsto> R \<heavy_comma> (a,b) \<tycolon> (A \<cross_product>' B) \<flower> W \<brangle>"
   unfolding AutoFusion_def by (rule call) (rule pr_\<nu>proc)
-lemma dpr_auto_schema: "\<^bold>p\<^bold>r\<^bold>o\<^bold>c call op_depair \<blangle> R \<heavy_comma> (a,b) \<tycolon> (A \<nuFusion>' B) \<flower> W \<longmapsto> R \<heavy_comma> a \<tycolon> A \<heavy_comma> b \<tycolon> B \<flower> W \<brangle>"
+lemma dpr_auto_schema: "\<^bold>p\<^bold>r\<^bold>o\<^bold>c call op_depair \<blangle> R \<heavy_comma> (a,b) \<tycolon> (A \<cross_product>' B) \<flower> W \<longmapsto> R \<heavy_comma> a \<tycolon> A \<heavy_comma> b \<tycolon> B \<flower> W \<brangle>"
   unfolding AutoFusion_def by (rule call) (rule dpr_\<nu>proc)
-lemma pr_auto_schema': "\<^bold>p\<^bold>r\<^bold>o\<^bold>c op_pair \<blangle> R \<heavy_comma> a \<tycolon> A \<heavy_comma> b \<tycolon> B \<longmapsto> R \<heavy_comma> (a,b) \<tycolon> (A \<nuFusion>' B) \<brangle>"
+lemma pr_auto_schema': "\<^bold>p\<^bold>r\<^bold>o\<^bold>c op_pair \<blangle> R \<heavy_comma> a \<tycolon> A \<heavy_comma> b \<tycolon> B \<longmapsto> R \<heavy_comma> (a,b) \<tycolon> (A \<cross_product>' B) \<brangle>"
   unfolding AutoFusion_def by (rule pr_\<nu>proc)
-lemma dpr_auto_schema': "\<^bold>p\<^bold>r\<^bold>o\<^bold>c op_depair \<blangle> R \<heavy_comma> (a,b) \<tycolon> (A \<nuFusion>' B) \<longmapsto> R \<heavy_comma> a \<tycolon> A \<heavy_comma> b \<tycolon> B \<brangle>"
+lemma dpr_auto_schema': "\<^bold>p\<^bold>r\<^bold>o\<^bold>c op_depair \<blangle> R \<heavy_comma> (a,b) \<tycolon> (A \<cross_product>' B) \<longmapsto> R \<heavy_comma> a \<tycolon> A \<heavy_comma> b \<tycolon> B \<brangle>"
   unfolding AutoFusion_def by (rule dpr_\<nu>proc)
 *)
 section \<open>Sugars\<close>
